ExistentialRules/AtomsAndRules/Atom.lean
@@ -23,23 +23,22 @@ namespace FunctionFreeAtom
 variable {sig : Signature} [DecidableEq sig.P] [DecidableEq sig.C] [DecidableEq sig.V]
 
 /-- We can `skolemize` a `FunctionFreeAtom` by skolemizing all its `VarOrConst`s. This yields an `Atom`. -/
-def skolemize (ruleId : Nat) (disjunctIndex : Nat) (frontier : List sig.V) (a : FunctionFreeAtom sig) : Atom sig := {
+def skolemize (rule : Rule sig) (i : Nat) (lt : i < rule.head.length) (a : FunctionFreeAtom sig) : Atom sig := {
   predicate := a.predicate,
-  terms := a.terms.map (VarOrConst.skolemize ruleId disjunctIndex frontier),
+  terms := a.terms.map (VarOrConst.skolemize rule i lt),
   arity_ok := by rw [List.length_map, a.arity_ok]
 }
 
 /-- The number of terms remains unchanged when Skolemizing. -/
 @[simp, grind =]
-theorem length_skolemize {ruleId : Nat} {disjunctIndex : Nat} {frontier : List sig.V} {a : FunctionFreeAtom sig} :
-    (a.skolemize ruleId disjunctIndex frontier).terms.length = a.terms.length := by
+theorem length_skolemize {rule : Rule sig} {i : Nat} {lt : i < rule.head.length} {a : FunctionFreeAtom sig} :
+    (a.skolemize rule i lt).terms.length = a.terms.length := by
   unfold skolemize; simp
 
 /-- If a a `VarOrConst` occurs in the terms of the `FunctionFreeAtom`, then the Skolemized `VarOrConst` occurs in the Skolemized `Atom`. -/
 @[grind <-]
-theorem mem_skolemize_of_mem {ruleId : Nat} {disjunctIndex : Nat} {frontier : List sig.V}
-    {a : FunctionFreeAtom sig} {t : VarOrConst sig} :
-    t ∈ a.terms -> (t.skolemize ruleId disjunctIndex frontier) ∈ (a.skolemize ruleId disjunctIndex frontier).terms := by
+theorem mem_skolemize_of_mem {rule : Rule sig} {i : Nat} {lt : i < rule.head.length} {a : FunctionFreeAtom sig} {t : VarOrConst sig} :
+    t ∈ a.terms -> (t.skolemize rule i lt) ∈ (a.skolemize rule i lt).terms := by
   unfold skolemize
   intro t_mem
   rw [List.mem_map]
