ExistentialRules/AtomsAndRules/RuleSet.lean
@@ -10,6 +10,7 @@ public import BasicLeanDatastructures.Set.Basic
 public import BasicLeanDatastructures.Set.Finite
 
 public import ExistentialRules.AtomsAndRules.Rule
+public import ExistentialRules.Terms.SkolemTerm
 
 
 /-!
@@ -18,47 +19,45 @@ public import ExistentialRules.AtomsAndRules.Rule
 
 public section
 
-/-- A `RuleSet` is a `Set (Rule sig)` where rules are uniquely identified by their id. -/
-structure RuleSet (sig : Signature) [DecidableEq sig.P] [DecidableEq sig.C] [DecidableEq sig.V] where
-  rules : Set (Rule sig)
-  id_unique : ∀ r1 r2, r1 ∈ rules ∧ r2 ∈ rules ∧ r1.id = r2.id -> r1 = r2
+/-- A `RuleSet` is a `Set (Rule sig)`. -/
+abbrev RuleSet (sig : Signature) [DecidableEq sig.P] [DecidableEq sig.C] [DecidableEq sig.V] := Set (Rule sig)
 
-/-- A `RuleList` is a `List (Rule sig)` where rules are uniquely identified by their id. -/
-structure RuleList (sig : Signature) [DecidableEq sig.P] [DecidableEq sig.C] [DecidableEq sig.V] where
-  rules : List (Rule sig)
-  id_unique : ∀ r1 r2, r1 ∈ rules ∧ r2 ∈ rules ∧ r1.id = r2.id -> r1 = r2
+/-- A `RuleList` is a `List (Rule sig)`. -/
+abbrev RuleList (sig : Signature) [DecidableEq sig.P] [DecidableEq sig.C] [DecidableEq sig.V] := List (Rule sig)
 
 namespace RuleSet
 
 /-!
 ## RuleSet
+
+For the `RuleSet` we introduce auxiliary definitions and theorems. For the `RuleList` we just use List functions directly.
 -/
 
 variable {sig : Signature} [DecidableEq sig.P] [DecidableEq sig.C] [DecidableEq sig.V]
 
 /-- A `RuleSet` is is deterministic if each rule is. -/
 @[expose]
-def isDeterministic (rs : RuleSet sig) : Prop := ∀ (r : Rule sig), r ∈ rs.rules -> r.isDeterministic
+def isDeterministic (rs : RuleSet sig) : Prop := ∀ (r : Rule sig), r ∈ rs -> r.isDeterministic
 
 /-- The predicate symbols of a `RuleSet` are the predicate symbols from all rules. -/
 @[expose]
-def predicates (rs : RuleSet sig) : Set sig.P := fun p => ∃ r, r ∈ rs.rules ∧ p ∈ r.predicates
+def predicates (rs : RuleSet sig) : Set sig.P := fun p => ∃ r, r ∈ rs ∧ p ∈ r.predicates
 
 /-- The constants of a `RuleSet` are the constants from all rules. -/
 @[expose]
-def constants (rs : RuleSet sig) : Set sig.C := fun c => ∃ r, r ∈ rs.rules ∧ c ∈ r.constants
+def constants (rs : RuleSet sig) : Set sig.C := fun c => ∃ r, r ∈ rs ∧ c ∈ r.constants
 
 /-- The head constants of a `RuleSet` are the head constants from all rules. -/
 @[expose]
-def head_constants (rs : RuleSet sig) : Set sig.C := fun c => ∃ r, r ∈ rs.rules ∧ c ∈ r.head_constants
+def head_constants (rs : RuleSet sig) : Set sig.C := fun c => ∃ r, r ∈ rs ∧ c ∈ r.head_constants
 
 /-- The Skolem function symbols of a `RuleSet` are the Skolem function symbols from all rules. -/
 @[expose]
-def skolem_functions (rs : RuleSet sig) : Set (SkolemFS sig) := fun f => ∃ r, r ∈ rs.rules ∧ f ∈ r.skolem_functions
+def skolem_functions (rs : RuleSet sig) : Set (SkolemFS sig) := fun f => ∃ r, r ∈ rs ∧ f ∈ r.skolem_functions
 
 /-- If the `RuleSet` is finite, so are the `RuleSet.predicates`. -/
 @[grind ->]
-theorem predicates_finite_of_finite (rs : RuleSet sig) : rs.rules.finite -> rs.predicates.finite := by
+theorem predicates_finite_of_finite (rs : RuleSet sig) : rs.finite -> rs.predicates.finite := by
   intro finite
   rcases finite with ⟨l, nodup, eq⟩
   exists (l.flatMap Rule.predicates).eraseDupsKeepRight
@@ -72,7 +71,7 @@ theorem predicates_finite_of_finite (rs : RuleSet sig) : rs.rules.finite -> rs.p
 
 /-- If the `RuleSet` is finite, so are the `RuleSet.constants`. -/
 @[grind ->]
-theorem constants_finite_of_finite (rs : RuleSet sig) : rs.rules.finite -> rs.constants.finite := by
+theorem constants_finite_of_finite (rs : RuleSet sig) : rs.finite -> rs.constants.finite := by
   intro finite
   rcases finite with ⟨l, nodup, eq⟩
   exists (l.flatMap Rule.constants).eraseDupsKeepRight
@@ -86,7 +85,7 @@ theorem constants_finite_of_finite (rs : RuleSet sig) : rs.rules.finite -> rs.co
 
 /-- If the `RuleSet` is finite, so are the `RuleSet.head_constants`. -/
 @[grind ->]
-theorem head_constants_finite_of_finite (rs : RuleSet sig) : rs.rules.finite -> rs.head_constants.finite := by
+theorem head_constants_finite_of_finite (rs : RuleSet sig) : rs.finite -> rs.head_constants.finite := by
   intro finite
   rcases finite with ⟨l, nodup, eq⟩
   exists (l.flatMap Rule.head_constants).eraseDupsKeepRight
@@ -100,7 +99,7 @@ theorem head_constants_finite_of_finite (rs : RuleSet sig) : rs.rules.finite -> 
 
 /-- If the `RuleSet` is finite, so are the `RuleSet.skolem_functions`. -/
 @[grind ->]
-theorem skolem_functions_finite_of_finite (rs : RuleSet sig) : rs.rules.finite -> rs.skolem_functions.finite := by
+theorem skolem_functions_finite_of_finite (rs : RuleSet sig) : rs.finite -> rs.skolem_functions.finite := by
   intro finite
   rcases finite with ⟨l, nodup, eq⟩
   exists (l.flatMap Rule.skolem_functions).eraseDupsKeepRight
@@ -123,35 +122,4 @@ theorem head_constants_subset_constants (rs : RuleSet sig) : rs.head_constants �
   . apply Rule.head_constants_subset_constants; exact c_mem
 
 end RuleSet
-
-namespace RuleList
-
-/-!
-## RuleList
--/
-
-variable {sig : Signature} [DecidableEq sig.P] [DecidableEq sig.C] [DecidableEq sig.V]
-
-/-- In a `RuleList`, we can obtain a rule based on its id. -/
-def get_by_id (rl : RuleList sig) (id : Nat) (id_mem : ∃ r ∈ rl.rules, r.id = id) : Rule sig :=
-  (rl.rules.find? (fun r => r.id = id)).get (by simp [id_mem])
-
-/-- A rule that we get by id is in the `RuleList`. -/
-theorem get_by_id_mem (rl : RuleList sig) (id : Nat) (id_mem : ∃ r ∈ rl.rules, r.id = id) : rl.get_by_id id id_mem ∈ rl.rules := by
-  unfold get_by_id; apply List.get_find?_mem
-
-/-- A rule that we get by id is indeed the rule that the id belongs to. -/
-@[simp, grind =]
-theorem get_by_id_self (rl : RuleList sig) (r : Rule sig) (mem : r ∈ rl.rules) : rl.get_by_id r.id (by exists r) = r := by
-  apply rl.id_unique
-  constructor
-  . apply List.get_find?_mem
-  constructor
-  . exact mem
-  . unfold get_by_id
-    have eq : rl.rules.find? (fun r' => r'.id = r.id) = some ((rl.rules.find? (fun r' => r'.id = r.id)).get (by rw [List.find?_isSome]; exists r; constructor; exact mem; simp)) := by simp
-    apply of_decide_eq_true
-    apply List.find?_some eq
-
-end RuleList
 
