ExistentialRules/ChaseSequence/Termination/BacktrackingOfFacts/PreGroundTerm.lean
@@ -19,66 +19,30 @@ variable {sig : Signature} [DecidableEq sig.P] [DecidableEq sig.C] [DecidableEq 
 
 namespace PreGroundTerm
 
-/-- `SkolemFS.ruleId_valid` lifted to `PreGroundTerm`. -/
-@[expose]
-def skolem_ruleIds_valid (rl : RuleList sig) : PreGroundTerm sig -> Prop
-| .leaf _ => True
-| .inner func ts => func.ruleId_valid rl ∧ ∀ t ∈ ts, PreGroundTerm.skolem_ruleIds_valid rl t
-
-/-- `SkolemFS.disjunctIndex_valid` lifted to `PreGroundTerm`. -/
-@[expose]
-def skolem_disjIdx_valid
-    (rl : RuleList sig)
-    (term : PreGroundTerm sig)
-    (term_ruleIds_valid : PreGroundTerm.skolem_ruleIds_valid rl term) : Prop :=
-  match term with
-  | .leaf _ => True
-  | .inner func ts =>
-    have : func.ruleId_valid rl ∧ ∀ t ∈ ts, PreGroundTerm.skolem_ruleIds_valid rl t := by unfold PreGroundTerm.skolem_ruleIds_valid at term_ruleIds_valid; exact term_ruleIds_valid
-    func.disjunctIndex_valid rl this.left ∧ ∀ t, (t_mem : t ∈ ts) -> PreGroundTerm.skolem_disjIdx_valid rl t (this.right t t_mem)
-
-/-- `SkolemFS.arity_valid` lifted to `PreGroundTerm`. -/
-@[expose]
-def skolem_rule_arity_valid
-    (rl : RuleList sig)
-    (term : PreGroundTerm sig)
-    (term_ruleIds_valid : PreGroundTerm.skolem_ruleIds_valid rl term) : Prop :=
-  match term with
-  | .leaf _ => True
-  | .inner func ts =>
-    have : func.ruleId_valid rl ∧ ∀ t ∈ ts, PreGroundTerm.skolem_ruleIds_valid rl t := by unfold PreGroundTerm.skolem_ruleIds_valid at term_ruleIds_valid; exact term_ruleIds_valid
-    func.arity_valid rl this.left ∧ ∀ t, (t_mem : t ∈ ts) -> PreGroundTerm.skolem_rule_arity_valid rl t (this.right t t_mem)
-
 /-- For a functional `PreGroundTerm`, we can find a `PreTrigger` that introduces it (while putting fresh constants for body variables). -/
 @[expose]
 def backtrackTrigger
     [GetFreshInhabitant sig.C]
     [Inhabited sig.C]
-    (rl : RuleList sig)
     (term : PreGroundTerm sig)
     (term_is_func : ∃ func ts, term = .inner func ts)
     (term_arity_ok : PreGroundTerm.arity_ok term)
-    (term_ruleIds_valid : PreGroundTerm.skolem_ruleIds_valid rl term)
-    (term_rule_arity_valid : PreGroundTerm.skolem_rule_arity_valid rl term term_ruleIds_valid)
     (forbidden_constants : List sig.C) :
     PreTrigger sig :=
   match term with
   | .leaf c => by simp at term_is_func -- contradiction
   | .inner func ts =>
-    let rule : Rule sig := rl.get_by_id func.ruleId (by unfold PreGroundTerm.skolem_ruleIds_valid at term_ruleIds_valid; exact term_ruleIds_valid.left)
-    let fresh_consts_for_pure_body_vars := rule.fresh_consts_for_pure_body_vars forbidden_constants
+    let fresh_consts_for_pure_body_vars := func.rule.fresh_consts_for_pure_body_vars forbidden_constants
 
     let subs : GroundSubstitution sig := fun x =>
-      if mem : x ∈ rule.frontier
+      if mem : x ∈ func.rule.frontier
       then
-        let idx := rule.frontier.idxOf x
+        let idx := func.rule.frontier.idxOf x
         have : idx < ts.length := by
           unfold arity_ok at term_arity_ok
-          unfold skolem_rule_arity_valid at term_rule_arity_valid
           have := LawfulBEq.eq_of_beq (Bool.and_eq_true_iff.mp term_arity_ok).left
-          rw [this, term_rule_arity_valid.left]
-          apply List.idxOf_lt_length_of_mem
-          exact mem
+          rw [this]; unfold SkolemFS.arity
+          exact List.idxOf_lt_length_of_mem mem
         ⟨ts[idx], by
           unfold arity_ok at term_arity_ok
           have := (Bool.and_eq_true_iff.mp term_arity_ok).right
@@ -87,9 +51,9 @@ def backtrackTrigger
           apply List.mem_attach
         ⟩
       else
-        if mem : x ∈ rule.pure_body_vars
+        if mem : x ∈ func.rule.pure_body_vars
         then
-          let idx := rule.pure_body_vars.idxOf x
+          let idx := func.rule.pure_body_vars.idxOf x
           have : idx < fresh_consts_for_pure_body_vars.val.length := by
             rw [fresh_consts_for_pure_body_vars.property.left]
             apply List.idxOf_lt_length_of_mem
@@ -99,7 +63,7 @@ def backtrackTrigger
           -- it should not matter what we return here so we also do NOT need to make sure that this does not collide with other constants
           GroundTerm.const default
 
-    { rule, subs }
+    { rule := func.rule, subs }
 
 -- This is not nicely possible without a mutual definition. The _list version is quite involved itself.
 mutual
@@ -109,12 +73,8 @@ mutual
   def backtrackFacts
       [GetFreshInhabitant sig.C]
       [Inhabited sig.C]
-      (rl : RuleList sig)
       (term : PreGroundTerm sig)
       (term_arity_ok : PreGroundTerm.arity_ok term)
-      (term_ruleIds_valid : PreGroundTerm.skolem_ruleIds_valid rl term)
-      (term_disjIdx_valid : PreGroundTerm.skolem_disjIdx_valid rl term term_ruleIds_valid)
-      (term_rule_arity_valid : PreGroundTerm.skolem_rule_arity_valid rl term term_ruleIds_valid)
       (forbidden_constants : List sig.C) :
       -- we return the backtracked facts and all the constants that have been freshly introduced (as a basis for picking other fresh ones)
       (List (Fact sig)) × (List sig.C) :=
@@ -122,23 +82,20 @@ mutual
     | .leaf c => ([], [])
     | .inner func ts =>
       have term_arity_ok' : ts.length == func.arity && ts.attach.all (fun ⟨t, _⟩ => arity_ok t) := by unfold arity_ok at term_arity_ok; exact term_arity_ok
-      have term_ruleIds_valid' : func.ruleId_valid rl ∧ ∀ t ∈ ts, PreGroundTerm.skolem_ruleIds_valid rl t := by unfold skolem_ruleIds_valid at term_ruleIds_valid; exact term_ruleIds_valid
-      have term_disjIdx_valid' : func.disjunctIndex_valid rl term_ruleIds_valid'.left ∧ ∀ t, (t_mem : t ∈ ts) -> PreGroundTerm.skolem_disjIdx_valid rl t (term_ruleIds_valid'.right t t_mem) := by unfold skolem_disjIdx_valid at term_disjIdx_valid; exact term_disjIdx_valid
-      have term_rule_arity_valid' : func.arity_valid rl term_ruleIds_valid'.left ∧ ∀ t, (t_mem : t ∈ ts) -> PreGroundTerm.skolem_rule_arity_valid rl t (term_ruleIds_valid'.right t t_mem) := by unfold skolem_rule_arity_valid at term_rule_arity_valid; exact term_rule_arity_valid
 
-      let trg : PreTrigger sig := backtrackTrigger rl (.inner func ts) (by exists func, ts) term_arity_ok term_ruleIds_valid term_rule_arity_valid forbidden_constants
-      let disjIdx := func.disjunctIndex
-      have : disjIdx < trg.mapped_head.length := by rw [PreTrigger.length_mapped_head]; unfold trg; unfold backtrackTrigger; exact term_disjIdx_valid'.left
+      let trg : PreTrigger sig := backtrackTrigger (.inner func ts) (by exists func, ts) term_arity_ok forbidden_constants
+      let disjIdx := func.headIdx
+      have : disjIdx < trg.mapped_head.length := by rw [PreTrigger.length_mapped_head]; exact func.headIdx_lt
 
       let fresh_consts_for_pure_body_vars := trg.rule.fresh_consts_for_pure_body_vars forbidden_constants
 
-      let res_ts := backtrackFacts_list rl ts (by
+      let res_ts := backtrackFacts_list ts (by
         intro t t_mem
         have := (Bool.and_eq_true_iff.mp term_arity_ok').right
         rw [List.all_eq_true] at this
         apply this ⟨t, t_mem⟩
         apply List.mem_attach
-      ) term_ruleIds_valid'.right term_disjIdx_valid'.right term_rule_arity_valid'.right (forbidden_constants ++ fresh_consts_for_pure_body_vars)
+      ) (forbidden_constants ++ fresh_consts_for_pure_body_vars)
 
       ((trg.mapped_body ++ trg.mapped_head[disjIdx]) ++ res_ts.fst, fresh_consts_for_pure_body_vars.val ++ res_ts.snd)
 
@@ -146,19 +103,15 @@ mutual
   def backtrackFacts_list
       [GetFreshInhabitant sig.C]
       [Inhabited sig.C]
-      (rl : RuleList sig)
       (terms : List (PreGroundTerm sig))
       (terms_arity_ok : ∀ t ∈ terms, PreGroundTerm.arity_ok t)
-      (terms_ruleIds_valid : ∀ t ∈ terms, PreGroundTerm.skolem_ruleIds_valid rl t)
-      (terms_disjIdx_valid : ∀ t, (t_mem : t ∈ terms) -> PreGroundTerm.skolem_disjIdx_valid rl t (terms_ruleIds_valid t t_mem))
-      (terms_rule_arity_valid : ∀ t, (t_mem : t ∈ terms) -> PreGroundTerm.skolem_rule_arity_valid rl t (terms_ruleIds_valid t t_mem))
       (forbidden_constants : List sig.C) :
       (List (Fact sig)) × (List sig.C) :=
     match terms with
     | .nil => ([], [])
     | .cons hd tl =>
-      let res_hd := backtrackFacts rl hd (terms_arity_ok hd (by simp)) (terms_ruleIds_valid hd (by simp)) (terms_disjIdx_valid hd (by simp)) (terms_rule_arity_valid hd (by simp)) forbidden_constants
-      let res_tl := backtrackFacts_list rl tl (by intro t t_mem; apply terms_arity_ok; simp [t_mem]) (by intro t t_mem; apply terms_ruleIds_valid; simp [t_mem])  (by intro t t_mem; apply terms_disjIdx_valid; simp [t_mem]) (by intro t t_mem; apply terms_rule_arity_valid; simp [t_mem]) (forbidden_constants ++ res_hd.snd)
+      let res_hd := backtrackFacts hd (terms_arity_ok hd (by simp)) forbidden_constants
+      let res_tl := backtrackFacts_list tl (by intro t t_mem; apply terms_arity_ok; simp [t_mem]) (forbidden_constants ++ res_hd.snd)
       (res_hd.fst ++ res_tl.fst, res_hd.snd ++ res_tl.snd)
 
 end
@@ -166,29 +119,19 @@ end
 theorem backtrackFacts_list_nil
     [GetFreshInhabitant sig.C]
     [Inhabited sig.C]
-    {rl : RuleList sig}
     {forbidden_constants : List sig.C} :
-    backtrackFacts_list rl [] (by simp) (by simp) (by simp) (by simp) forbidden_constants = ([], []) := by simp [backtrackFacts_list]
+    backtrackFacts_list [] (by simp) forbidden_constants = ([], []) := by simp [backtrackFacts_list]
 
 theorem backtrackFacts_list_cons
     [GetFreshInhabitant sig.C]
     [Inhabited sig.C]
-    {rl : RuleList sig}
     {term : PreGroundTerm sig}
     {terms : List (PreGroundTerm sig)}
     {terms_arity_ok : ∀ t ∈ (term :: terms), PreGroundTerm.arity_ok t}
-    {terms_ruleIds_valid : ∀ t ∈ (term :: terms), PreGroundTerm.skolem_ruleIds_valid rl t}
-    {terms_disjIdx_valid : ∀ t, (t_mem : t ∈ (term :: terms)) -> PreGroundTerm.skolem_disjIdx_valid rl t (terms_ruleIds_valid t t_mem)}
-    {terms_rule_arity_valid : ∀ t, (t_mem : t ∈ (term :: terms)) -> PreGroundTerm.skolem_rule_arity_valid rl t (terms_ruleIds_valid t t_mem)}
     {forbidden_constants : List sig.C} :
-    backtrackFacts_list rl (term :: terms) terms_arity_ok terms_ruleIds_valid terms_disjIdx_valid terms_rule_arity_valid forbidden_constants =
-      let res_t := backtrackFacts rl term (by apply terms_arity_ok; simp) (by apply terms_ruleIds_valid; simp) (by apply terms_disjIdx_valid; simp) (by apply terms_rule_arity_valid; simp) forbidden_constants
-      let res_ts := backtrackFacts_list rl terms
-        (by intro t t_mem; apply terms_arity_ok; simp [t_mem])
-        (by intro t t_mem; apply terms_ruleIds_valid; simp [t_mem])
-        (by intro t t_mem; apply terms_disjIdx_valid; simp [t_mem])
-        (by intro t t_mem; apply terms_rule_arity_valid; simp [t_mem])
-        (forbidden_constants ++ res_t.snd)
+    backtrackFacts_list (term :: terms) terms_arity_ok forbidden_constants =
+      let res_t := backtrackFacts term (by apply terms_arity_ok; simp) forbidden_constants
+      let res_ts := backtrackFacts_list terms (by intro t t_mem; apply terms_arity_ok; simp [t_mem]) (forbidden_constants ++ res_t.snd)
       (res_t.fst ++ res_ts.fst, res_t.snd ++ res_ts.snd) := by rfl
 
 -- It's good to have this as mutual since we need the result on lists anyway.
@@ -198,14 +141,10 @@ mutual
   theorem backtrackFacts_fresh_constants_not_forbidden
       [GetFreshInhabitant sig.C]
       [Inhabited sig.C]
-      {rl : RuleList sig}
       {term : PreGroundTerm sig}
       {term_arity_ok : PreGroundTerm.arity_ok term}
-      {term_ruleIds_valid : PreGroundTerm.skolem_ruleIds_valid rl term}
-      {term_disjIdx_valid : PreGroundTerm.skolem_disjIdx_valid rl term term_ruleIds_valid}
-      {term_rule_arity_valid : PreGroundTerm.skolem_rule_arity_valid rl term term_ruleIds_valid}
       {forbidden_constants : List sig.C} :
-      ∀ c ∈ (PreGroundTerm.backtrackFacts rl term term_arity_ok term_ruleIds_valid term_disjIdx_valid term_rule_arity_valid forbidden_constants).snd, c ∉ forbidden_constants := by
+      ∀ c ∈ (PreGroundTerm.backtrackFacts term term_arity_ok forbidden_constants).snd, c ∉ forbidden_constants := by
     intro c c_mem
     cases term with
     | leaf _ => simp [backtrackFacts] at c_mem
@@ -214,7 +153,7 @@ mutual
       rw [List.mem_append] at c_mem
       cases c_mem with
       | inl c_mem =>
-        let trg : PreTrigger sig := backtrackTrigger rl (.inner func ts) (by exists func, ts) term_arity_ok term_ruleIds_valid term_rule_arity_valid forbidden_constants
+        let trg : PreTrigger sig := backtrackTrigger (.inner func ts) (by exists func, ts) term_arity_ok forbidden_constants
         let fresh_consts_for_pure_body_vars := trg.rule.fresh_consts_for_pure_body_vars forbidden_constants
         apply fresh_consts_for_pure_body_vars.property.right.right
         exact c_mem
@@ -223,14 +162,10 @@ mutual
   theorem backtrackFacts_list_fresh_constants_not_forbidden
       [GetFreshInhabitant sig.C]
       [Inhabited sig.C]
-      {rl : RuleList sig}
       {terms : List (PreGroundTerm sig)}
       {terms_arity_ok : ∀ t ∈ terms, PreGroundTerm.arity_ok t}
-      {terms_ruleIds_valid : ∀ t ∈ terms, PreGroundTerm.skolem_ruleIds_valid rl t}
-      {terms_disjIdx_valid : ∀ t, (t_mem : t ∈ terms) -> PreGroundTerm.skolem_disjIdx_valid rl t (terms_ruleIds_valid t t_mem)}
-      {terms_rule_arity_valid : ∀ t, (t_mem : t ∈ terms) -> PreGroundTerm.skolem_rule_arity_valid rl t (terms_ruleIds_valid t t_mem)}
       {forbidden_constants : List sig.C} :
-      ∀ c ∈ (PreGroundTerm.backtrackFacts_list rl terms terms_arity_ok terms_ruleIds_valid terms_disjIdx_valid terms_rule_arity_valid forbidden_constants).snd, c ∉ forbidden_constants := by
+      ∀ c ∈ (PreGroundTerm.backtrackFacts_list terms terms_arity_ok forbidden_constants).snd, c ∉ forbidden_constants := by
     intro c c_mem
     cases terms with
     | nil => simp [backtrackFacts_list_nil] at c_mem
@@ -252,16 +187,12 @@ mutual
   theorem backtrackFacts_constants_in_rules_or_term_or_fresh
       [GetFreshInhabitant sig.C]
       [Inhabited sig.C]
-      {rl : RuleList sig}
       {term : PreGroundTerm sig}
       {term_arity_ok : PreGroundTerm.arity_ok term}
-      {term_ruleIds_valid : PreGroundTerm.skolem_ruleIds_valid rl term}
-      {term_disjIdx_valid : PreGroundTerm.skolem_disjIdx_valid rl term term_ruleIds_valid}
-      {term_rule_arity_valid : PreGroundTerm.skolem_rule_arity_valid rl term term_ruleIds_valid}
       {forbidden_constants : List sig.C} :
-      ∀ f ∈ (PreGroundTerm.backtrackFacts rl term term_arity_ok term_ruleIds_valid term_disjIdx_valid term_rule_arity_valid forbidden_constants).fst,
+      ∀ f ∈ (PreGroundTerm.backtrackFacts term term_arity_ok forbidden_constants).fst,
       ∀ c ∈ f.constants,
-        c ∈ (rl.rules.flatMap Rule.constants) ∨ c ∈ term.leaves ∨ c ∈ (PreGroundTerm.backtrackFacts rl term term_arity_ok term_ruleIds_valid term_disjIdx_valid term_rule_arity_valid forbidden_constants).snd := by
+        c ∈ (term.innerLabels.flatMap (Rule.constants ∘ SkolemFS.rule)) ∨ c ∈ term.leaves ∨ c ∈ (PreGroundTerm.backtrackFacts term term_arity_ok forbidden_constants).snd := by
     intro f f_mem c c_mem
     cases term with
     | leaf _ => simp [backtrackFacts] at f_mem
@@ -270,7 +201,7 @@ mutual
       rw [List.mem_append] at f_mem
       cases f_mem with
       | inl f_mem =>
-        let trg := backtrackTrigger rl (.inner func ts) (by exists func, ts) term_arity_ok term_ruleIds_valid term_rule_arity_valid forbidden_constants
+        let trg := backtrackTrigger (.inner func ts) (by exists func, ts) term_arity_ok forbidden_constants
         rw [List.mem_append] at f_mem
         cases f_mem with
         | inl f_mem =>
@@ -284,11 +215,11 @@ mutual
             rcases t_mem with ⟨d, d_mem, t_eq⟩
             apply Or.inl
             rw [List.mem_flatMap]
-            exists trg.rule
+            exists func
             constructor
-            . simp only [trg, backtrackTrigger]
-              apply RuleList.get_by_id_mem
-            . unfold Rule.constants
+            . simp [FiniteTree.innerLabels]
+            . rw [Function.comp_apply]
+              unfold Rule.constants
               rw [List.mem_append]
               apply Or.inl
               rw [← t_eq, GroundTerm.constants_const, List.mem_singleton] at c_mem
@@ -332,9 +263,9 @@ mutual
               rw [c_mem]
               apply List.getElem_mem
         | inr f_mem =>
-          have disjIdx_lt : func.disjunctIndex < trg.mapped_head.length := by rw [PreTrigger.length_mapped_head]; unfold skolem_disjIdx_valid at term_disjIdx_valid; apply term_disjIdx_valid.left
-          have c_mem : c ∈ FactSet.constants trg.mapped_head[func.disjunctIndex].toSet := by exists f; rw [List.mem_toSet]; exact ⟨f_mem, c_mem⟩
-          have c_mem := trg.mapped_head_constants_subset ⟨func.disjunctIndex, disjIdx_lt⟩ c c_mem
+          have headIdx_lt : func.headIdx < trg.mapped_head.length := by rw [PreTrigger.length_mapped_head]; exact func.headIdx_lt
+          have c_mem : c ∈ FactSet.constants trg.mapped_head[func.headIdx].toSet := by exists f; rw [List.mem_toSet]; exact ⟨f_mem, c_mem⟩
+          have c_mem := trg.mapped_head_constants_subset func.headIdx func.headIdx_lt c c_mem
           rw [List.mem_toSet, List.mem_append] at c_mem
           cases c_mem with
           | inl c_mem =>
@@ -345,7 +276,7 @@ mutual
             rw [List.mem_map] at t_mem
             rcases t_mem with ⟨v, v_mem, t_eq⟩
             unfold PreTrigger.subs_for_mapped_head at t_eq
-            rw [PreTrigger.apply_to_var_or_const_frontier_var _ _ v v_mem] at t_eq
+            rw [PreTrigger.apply_to_var_or_const_frontier_var _ _ _ v v_mem] at t_eq
             simp only [trg, backtrackTrigger] at v_mem
             simp only [trg, backtrackTrigger, v_mem, ↓reduceDIte] at t_eq
             rw [← t_eq] at c_mem
@@ -360,22 +291,22 @@ mutual
           | inr c_mem =>
             apply Or.inl
             rw [List.mem_flatMap]
-            exists trg.rule
+            exists func
             constructor
-            . simp only [trg, backtrackTrigger]
-              apply RuleList.get_by_id_mem
-            . unfold Rule.constants
+            . simp [FiniteTree.innerLabels]
+            . rw [Function.comp_apply]
+              unfold Rule.constants
               rw [List.mem_append]
               apply Or.inr
               rw [List.mem_flatMap]
-              exists trg.rule.head[func.disjunctIndex]'(by rw [← PreTrigger.length_mapped_head]; exact disjIdx_lt)
+              exists trg.rule.head[func.headIdx]'(func.headIdx_lt)
               constructor
               . apply List.getElem_mem
               . exact c_mem
       | inr f_mem =>
         simp only [FiniteTree.leaves, PreGroundTerm.backtrackFacts]
         cases PreGroundTerm.backtrackFacts_list_constants_in_rules_or_term_or_fresh f f_mem c c_mem with
-        | inl c_mem => apply Or.inl; exact c_mem
+        | inl c_mem => apply Or.inl; unfold FiniteTree.innerLabels; rw [List.flatMap_cons]; apply List.mem_append_right; exact c_mem
         | inr c_mem =>
           apply Or.inr
           cases c_mem with
@@ -385,16 +316,12 @@ mutual
   theorem backtrackFacts_list_constants_in_rules_or_term_or_fresh
       [GetFreshInhabitant sig.C]
       [Inhabited sig.C]
-      {rl : RuleList sig}
       {terms : List (PreGroundTerm sig)}
       {terms_arity_ok : ∀ t ∈ terms, PreGroundTerm.arity_ok t}
-      {terms_ruleIds_valid : ∀ t ∈ terms, PreGroundTerm.skolem_ruleIds_valid rl t}
-      {terms_disjIdx_valid : ∀ t, (t_mem : t ∈ terms) -> PreGroundTerm.skolem_disjIdx_valid rl t (terms_ruleIds_valid t t_mem)}
-      {terms_rule_arity_valid : ∀ t, (t_mem : t ∈ terms) -> PreGroundTerm.skolem_rule_arity_valid rl t (terms_ruleIds_valid t t_mem)}
       {forbidden_constants : List sig.C} :
-      ∀ f ∈ (PreGroundTerm.backtrackFacts_list rl terms terms_arity_ok terms_ruleIds_valid terms_disjIdx_valid terms_rule_arity_valid forbidden_constants).fst,
+      ∀ f ∈ (PreGroundTerm.backtrackFacts_list terms terms_arity_ok forbidden_constants).fst,
       ∀ c ∈ f.constants,
-        c ∈ (rl.rules.flatMap Rule.constants) ∨ c ∈ terms.flatMap FiniteTree.leaves ∨ c ∈ (PreGroundTerm.backtrackFacts_list rl terms terms_arity_ok terms_ruleIds_valid terms_disjIdx_valid terms_rule_arity_valid forbidden_constants).snd := by
+        c ∈ ((terms.flatMap FiniteTree.innerLabels).flatMap (Rule.constants ∘ SkolemFS.rule)) ∨ c ∈ terms.flatMap FiniteTree.leaves ∨ c ∈ (PreGroundTerm.backtrackFacts_list terms terms_arity_ok forbidden_constants).snd := by
     intro f f_mem c c_mem
     cases terms with
     | nil => simp [backtrackFacts_list] at f_mem
@@ -404,7 +331,7 @@ mutual
       cases f_mem with
       | inl f_mem =>
         cases PreGroundTerm.backtrackFacts_constants_in_rules_or_term_or_fresh f f_mem c c_mem with
-        | inl c_mem => apply Or.inl; exact c_mem
+        | inl c_mem => apply Or.inl; rw [List.flatMap_cons, List.flatMap_append]; apply List.mem_append_left; exact c_mem
         | inr c_mem =>
           apply Or.inr
           cases c_mem with
@@ -412,7 +339,7 @@ mutual
           | inr c_mem => apply Or.inr; simp only [backtrackFacts_list]; rw [List.mem_append]; apply Or.inl; exact c_mem
       | inr f_mem =>
         cases PreGroundTerm.backtrackFacts_list_constants_in_rules_or_term_or_fresh f f_mem c c_mem with
-        | inl c_mem => apply Or.inl; exact c_mem
+        | inl c_mem => apply Or.inl; rw [List.flatMap_cons, List.flatMap_append]; apply List.mem_append_right; exact c_mem
         | inr c_mem =>
           apply Or.inr
           cases c_mem with
