ExistentialRules/Triggers/Basic.lean
@@ -33,86 +33,124 @@ namespace PreTrigger
 
 variable {sig : Signature} [DecidableEq sig.P] [DecidableEq sig.C] [DecidableEq sig.V]
 
-/-- In the context of a trigger, we Skolemize a `VarOrConst` by passing the rule id and frontier of the rule in the trigger. -/
-def skolemize_var_or_const (trg : PreTrigger sig) (disjunctIndex : Nat) (var_or_const : VarOrConst sig) : SkolemTerm sig :=
-  var_or_const.skolemize trg.rule.id disjunctIndex trg.rule.frontier
+/-- In the context of a trigger, we Skolemize a `VarOrConst` by passing the rule in the trigger. -/
+def skolemize_var_or_const (trg : PreTrigger sig) (i : Nat) (lt : i < trg.rule.head.length) (var_or_const : VarOrConst sig) : SkolemTerm sig :=
+  var_or_const.skolemize trg.rule i lt
 
 /-- We apply a trigger to a `VarOrConst` by Skolemizing and then applying the `GroundSubstitution` from the trigger. We need this to define the trigger result later. -/
-def apply_to_var_or_const (trg : PreTrigger sig) (disjunctIndex : Nat) : TermMapping (VarOrConst sig) (GroundTerm sig) :=
-  (trg.subs.apply_skolem_term ∘ (trg.skolemize_var_or_const disjunctIndex))
+def apply_to_var_or_const (trg : PreTrigger sig) (i : Nat) (lt : i < trg.rule.head.length) : TermMapping (VarOrConst sig) (GroundTerm sig) :=
+  (trg.subs.apply_skolem_term ∘ (trg.skolemize_var_or_const i lt))
 
 /-- Applying a trigger to a constant changes nothing. -/
 @[simp, grind =]
-theorem apply_to_var_or_const_for_const (trg : PreTrigger sig) (i : Nat) :
-    ∀ c, trg.apply_to_var_or_const i (.const c) = GroundTerm.const c := by
+theorem apply_to_var_or_const_for_const (trg : PreTrigger sig) (i : Nat) (lt : i < trg.rule.head.length) :
+    ∀ c, trg.apply_to_var_or_const i lt (.const c) = GroundTerm.const c := by
   simp [apply_to_var_or_const, skolemize_var_or_const, VarOrConst.skolemize, GroundSubstitution.apply_skolem_term]
+
+/-- Applying a trigger to an non-existential variable does not skolemize but merely applied the substitution. -/
+@[simp, grind =]
+theorem apply_to_var_or_const_of_not_mem_existential_vars (trg : PreTrigger sig) (i : Nat) (lt : i < trg.rule.head.length) :
+    ∀ v, v ∉ trg.rule.existential_vars_for_head_disjunct i lt -> trg.apply_to_var_or_const i lt (.var v) = trg.subs v := by
+  intro v v_mem
+  simp [apply_to_var_or_const, skolemize_var_or_const, VarOrConst.skolemize, v_mem, GroundSubstitution.apply_skolem_term]
 
 /-- Applying a trigger to a frontier variable does not skolemize but merely applied the substitution. -/
 @[simp, grind =]
-theorem apply_to_var_or_const_frontier_var (trg : PreTrigger sig) (i : Nat) :
-    ∀ v, v ∈ trg.rule.frontier -> trg.apply_to_var_or_const i (.var v) = trg.subs v := by
+theorem apply_to_var_or_const_frontier_var (trg : PreTrigger sig) (i : Nat) (lt : i < trg.rule.head.length) :
+    ∀ v, v ∈ trg.rule.frontier -> trg.apply_to_var_or_const i lt (.var v) = trg.subs v := by
   intro v v_front
-  simp [apply_to_var_or_const, skolemize_var_or_const, VarOrConst.skolemize, v_front, GroundSubstitution.apply_skolem_term]
+  suffices v ∉ trg.rule.existential_vars_for_head_disjunct i lt by exact apply_to_var_or_const_of_not_mem_existential_vars _ _ _ _ this
+  intro contra; apply trg.rule.not_mem_frontier_of_mem_existential_vars_for_head_disjunct _ contra; exact v_front
 
 /-- A shortcut definition for how the Skolem term resulting from applying the trigger to an existential variable will look. -/
 @[expose]
-def functional_term_for_var (trg : PreTrigger sig) (i : Nat) (v : sig.V) : GroundTerm sig :=
+def functional_term_for_var
+    (trg : PreTrigger sig)
+    (i : Nat) (lt : i < trg.rule.head.length)
+    (v : sig.V)
+    (v_mem : v ∈ trg.rule.existential_vars_for_head_disjunct i lt) :
+    GroundTerm sig :=
   GroundTerm.func
-    { ruleId := trg.rule.id, disjunctIndex := i, var := v, arity := trg.rule.frontier.length }
+    { rule := trg.rule, headIdx := i, headIdx_lt := lt, v, v_mem }
     (trg.rule.frontier.map trg.subs)
-    (by rw [List.length_map])
+    (by rw [List.length_map]; rfl)
 
 /-- The `functional_term_for_var` function is injective for a fixed trigger. -/
 @[grind ->]
-theorem functional_term_for_var.inj {trg : PreTrigger sig} {i1 i2 : Nat} {v1 v2 : sig.V} :
-  trg.functional_term_for_var i1 v1 = trg.functional_term_for_var i2 v2 -> i1 = i2 ∧ v1 = v2 := by unfold functional_term_for_var; simp
+theorem functional_term_for_var.inj
+    {trg : PreTrigger sig} {i1 i2 : Nat} {lt1 : i1 < trg.rule.head.length} {lt2 : i2 < trg.rule.head.length}
+    {v1 : sig.V}
+    {v1_mem : v1 ∈ trg.rule.existential_vars_for_head_disjunct i1 lt1}
+    {v2 : sig.V}
+    {v2_mem : v2 ∈ trg.rule.existential_vars_for_head_disjunct i2 lt2} :
+    trg.functional_term_for_var i1 lt1 v1 v1_mem = trg.functional_term_for_var i2 lt2 v2 v2_mem -> i1 = i2 ∧ v1 = v2 := by
+  unfold functional_term_for_var; grind
 @[simp, grind =]
-theorem functional_term_for_var.injEq {trg : PreTrigger sig} {i1 i2 : Nat} {v1 v2 : sig.V} :
-  trg.functional_term_for_var i1 v1 = trg.functional_term_for_var i2 v2 ↔ i1 = i2 ∧ v1 = v2 := by unfold functional_term_for_var; simp
+theorem functional_term_for_var.injEq
+    {trg : PreTrigger sig} {i1 i2 : Nat} {lt1 : i1 < trg.rule.head.length} {lt2 : i2 < trg.rule.head.length}
+    {v1 : sig.V}
+    {v1_mem : v1 ∈ trg.rule.existential_vars_for_head_disjunct i1 lt1}
+    {v2 : sig.V}
+    {v2_mem : v2 ∈ trg.rule.existential_vars_for_head_disjunct i2 lt2} :
+    trg.functional_term_for_var i1 lt1 v1 v1_mem = trg.functional_term_for_var i2 lt2 v2 v2_mem ↔ i1 = i2 ∧ v1 = v2 := by
+  unfold functional_term_for_var; grind
 
-/-- Applying a trigger to a non-frontier variable, yields exactly the Skolem function term from the shortcup definition `functional_term_for_var`. -/
+/-- Applying a trigger to an existential variable, yields exactly the Skolem function term from the shortcup definition `functional_term_for_var`. -/
 @[simp, grind =]
-theorem apply_to_var_or_const_non_frontier_var (trg : PreTrigger sig) (i : Nat) :
-    ∀ v, ¬ v ∈ trg.rule.frontier -> trg.apply_to_var_or_const i (.var v) = trg.functional_term_for_var i v := by
-  intro v v_front
-  simp [functional_term_for_var, apply_to_var_or_const, skolemize_var_or_const, VarOrConst.skolemize, v_front, GroundSubstitution.apply_skolem_term]
+theorem apply_to_var_or_const_of_mem_existential_vars (trg : PreTrigger sig) (i : Nat) (lt : i < trg.rule.head.length) :
+    ∀ v, (mem : v ∈ trg.rule.existential_vars_for_head_disjunct i lt) ->
+    trg.apply_to_var_or_const i lt (.var v) = trg.functional_term_for_var i lt v mem := by
+  intro v v_mem
+  simp [functional_term_for_var, apply_to_var_or_const, skolemize_var_or_const, VarOrConst.skolemize, v_mem, GroundSubstitution.apply_skolem_term]
 
-/-- For non-frontier variable, applyign the trigger is injective. -/
-theorem apply_to_var_or_const_injective_of_not_in_frontier {v : sig.V}
-    (trg : PreTrigger sig) (i : Fin trg.rule.head.length) (v_not_in_frontier : ¬ v ∈ trg.rule.frontier) :
-    ∀ voc, (trg.apply_to_var_or_const i (VarOrConst.var v)) = (trg.apply_to_var_or_const i voc) -> VarOrConst.var v = voc := by
-  intro voc apply_eq
+/-- For existential variables, applying the trigger is injective. -/
+theorem apply_to_var_or_const_injective_of_mem_existential_vars {v : sig.V}
+    (trg : PreTrigger sig) (i : Nat) (lt : i < trg.rule.head.length) (v_mem : v ∈ trg.rule.existential_vars_for_head_disjunct i lt) :
+    ∀ voc ∈ trg.rule.head[i].terms, (trg.apply_to_var_or_const i lt (VarOrConst.var v)) = (trg.apply_to_var_or_const i lt voc) -> VarOrConst.var v = voc := by
+  intro voc voc_mem apply_eq
   cases voc with
-  | const c => simp [v_not_in_frontier, functional_term_for_var, GroundTerm.func_neq_const] at apply_eq
+  | const c => simp [v_mem, functional_term_for_var, GroundTerm.func_neq_const] at apply_eq
   | var u =>
-    cases Decidable.em (u ∈ trg.rule.frontier) with
-    | inl u_front =>
+    cases Decidable.em (u ∈ trg.rule.existential_vars_for_head_disjunct i lt) with
+    | inl u_mem => grind
+    | inr u_mem =>
       apply False.elim
-      rw [apply_to_var_or_const_non_frontier_var _ _ _ v_not_in_frontier, apply_to_var_or_const_frontier_var _ _ _ u_front] at apply_eq
+      rw [apply_to_var_or_const_of_mem_existential_vars _ _ _ _ v_mem, apply_to_var_or_const_of_not_mem_existential_vars _ _ _ _ u_mem] at apply_eq
       unfold functional_term_for_var at apply_eq
+      have u_front : u ∈ trg.rule.frontier := by
+        unfold Rule.existential_vars_for_head_disjunct at u_mem; rw [List.mem_filter, not_and, decide_not, not_decide_eq_true, Decidable.not_not] at u_mem
+        apply u_mem
+        rw [FunctionFreeConjunction.mem_vars']
+        exact voc_mem
       have : trg.subs u ∈ trg.rule.frontier.map trg.subs := List.mem_map_of_mem u_front
       rw [← apply_eq] at this
       exact GroundTerm.eq_while_contained_is_impossible this
-    | inr u_front => grind
 
 /-- Applying the trigger to non-frontier variables yields a term that cannot possibly be in the mapped frontier. In other words, terms for existential variables are fresh (although freshness entails more than that). -/
-theorem result_term_not_in_frontier_image_of_var_not_in_frontier (trg : PreTrigger sig)
-    (disj_index : Fin trg.rule.head.length) (v : sig.V) (v_not_in_frontier : ¬ v ∈ trg.rule.frontier) :
-    ¬ trg.apply_to_var_or_const disj_index.val (VarOrConst.var v) ∈ trg.rule.frontier.map trg.subs := by
+theorem result_term_not_in_frontier_image_of_var_existential (trg : PreTrigger sig) (i : Nat) (lt : i < trg.rule.head.length)
+    (v : sig.V) (v_existential : v ∈ trg.rule.existential_vars_for_head_disjunct i lt) :
+    ¬ trg.apply_to_var_or_const i lt (VarOrConst.var v) ∈ (trg.rule.frontier).map trg.subs := by
   intro contra
-  apply v_not_in_frontier
   rw [List.mem_map] at contra
   rcases contra with ⟨u, u_in_frontier, u_eq⟩
-  have := trg.apply_to_var_or_const_injective_of_not_in_frontier disj_index v_not_in_frontier (VarOrConst.var u)
-  grind
+  rw [apply_to_var_or_const_of_mem_existential_vars _ _ _ _ v_existential] at u_eq
+  unfold functional_term_for_var at u_eq
+  have : trg.subs u ∈ trg.rule.frontier.map trg.subs := List.mem_map_of_mem u_in_frontier
+  rw [u_eq] at this
+  exact GroundTerm.eq_while_contained_is_impossible this
 
 /-- We lift the trigger application from `VarOrConst` to `FunctionFreeAtom`. -/
-abbrev apply_to_function_free_atom (trg : PreTrigger sig) (disjunctIndex : Nat) (atom : FunctionFreeAtom sig) : Fact sig :=
-  (trg.apply_to_var_or_const disjunctIndex).apply_generalized_atom atom
+abbrev apply_to_function_free_atom (trg : PreTrigger sig) (i : Nat) (lt : i < trg.rule.head.length) (atom : FunctionFreeAtom sig) : Fact sig :=
+  (trg.apply_to_var_or_const i lt).apply_generalized_atom atom
 
 /-- The body does not feature any existential variables. Therefore, we mapped body merely results from applying the trigger's substitution to the body of its rule. -/
 @[expose]
 def mapped_body (trg : PreTrigger sig) : List (Fact sig) := trg.subs.apply_function_free_conj trg.rule.body
+
+/-- The length of the `mapped_body` is the same as the length of the rule body. -/
+@[simp, grind =]
+theorem length_mapped_body (trg : PreTrigger sig) : trg.mapped_body.length = trg.rule.body.length := by
+  simp [mapped_body, GroundSubstitution.apply_function_free_conj, TermMapping.apply_generalized_atom_list]
 
 /-- A term occurs in `mapped_body` if and only if it is a constant in the rule body of if there exists a variable in the rule body that is mapped to the term by the substitution. -/
 theorem mem_terms_mapped_body_iff (trg : PreTrigger sig) :
@@ -166,30 +204,29 @@ theorem mem_terms_mapped_body_iff (trg : PreTrigger sig) :
 /-- The mapped head is the result of the trigger and is simply the application to all head atoms. This result has a list of result facts for each of the head disjuncts. Note again that existential variables are Skolemized before the trigger's substitution is applied but this is hidden within the previously defined functions. -/
 @[expose]
 def mapped_head (trg : PreTrigger sig) : List (List (Fact sig)) :=
-  trg.rule.head.zipIdx.map (fun (h, i) => h.map (trg.apply_to_function_free_atom i))
+  trg.rule.head.zipIdx.attach.map (fun pair => pair.val.fst.map (trg.apply_to_function_free_atom pair.val.snd (List.snd_lt_of_mem_zipIdx pair.property)))
 
 /-- The length of the `mapped_head` is the same as the length of the rule head. That is, the trigger result indeed has one list of facts for each of the head disjuncts. -/
 @[simp, grind =]
 theorem length_mapped_head (trg : PreTrigger sig) : trg.mapped_head.length = trg.rule.head.length := by
-  unfold mapped_head
-  rw [List.length_map, List.length_zipIdx]
+  unfold mapped_head; simp
 
 /-- Also for each head disjunct, the number of result facts is equal to the number of atoms in the conjunction. -/
 theorem length_each_mapped_head (trg : PreTrigger sig) : ∀ (n : Nat), trg.mapped_head[n]?.map (List.length) = trg.rule.head[n]?.map (List.length) := by
   intro n
   unfold mapped_head
-  simp only [List.getElem?_map, List.getElem?_zipIdx, Option.map_map]
-  cases trg.rule.head[n]? <;> simp
+  simp only [List.getElem?_map, Option.map_map]
+  cases eq : trg.rule.head[n]? <;> grind
 
 /-- For a fixed head index, we can view the trigger merely as a substitution that internally captures the Skolemization of existential variables. In other words, applying this substitution to the specified head disjunct yields exactly the trigger result for the same disjunct. Viewing the trigger as a substitution can be convenient for theorems and proofs. -/
 @[expose]
-def subs_for_mapped_head (trg : PreTrigger sig) (i : Fin trg.mapped_head.length) : GroundSubstitution sig :=
-  fun v => trg.apply_to_var_or_const i (.var v)
+def subs_for_mapped_head (trg : PreTrigger sig) (i : Nat) (lt : i < trg.rule.head.length) : GroundSubstitution sig :=
+  fun v => trg.apply_to_var_or_const i lt (.var v)
 
 /-- Applying the `subs_for_mapped_head` is the same as applying the trigger on `VarOrConst`. -/
 @[simp, grind =]
-theorem apply_subs_for_var_or_const_eq (trg : PreTrigger sig) (i : Fin trg.mapped_head.length) :
-    ∀ voc, (trg.subs_for_mapped_head i).apply_var_or_const voc = trg.apply_to_var_or_const i voc := by
+theorem apply_subs_for_var_or_const_eq (trg : PreTrigger sig) (i : Nat) (lt : i < trg.rule.head.length) :
+    ∀ voc, (trg.subs_for_mapped_head i lt).apply_var_or_const voc = trg.apply_to_var_or_const i lt voc := by
   intro voc
   unfold GroundSubstitution.apply_var_or_const
   unfold subs_for_mapped_head
@@ -197,8 +234,8 @@ theorem apply_subs_for_var_or_const_eq (trg : PreTrigger sig) (i : Fin trg.mappe
 
 /-- Applying the `subs_for_mapped_head` is the same as applying the trigger on `FunctionFreeAtom`. -/
 @[simp, grind =]
-theorem apply_subs_for_atom_eq (trg : PreTrigger sig) (i : Fin trg.mapped_head.length) :
-    ∀ a, (trg.subs_for_mapped_head i).apply_function_free_atom a = trg.apply_to_function_free_atom i a := by
+theorem apply_subs_for_atom_eq (trg : PreTrigger sig) (i : Nat) (lt : i < trg.rule.head.length) :
+    ∀ a, (trg.subs_for_mapped_head i lt).apply_function_free_atom a = trg.apply_to_function_free_atom i lt a := by
   intro a
   unfold GroundSubstitution.apply_function_free_atom
   unfold apply_to_function_free_atom
@@ -208,29 +245,33 @@ theorem apply_subs_for_atom_eq (trg : PreTrigger sig) (i : Fin trg.mapped_head.l
 
 /-- Applying the `subs_for_mapped_head` on the head is exactly the trigger result (`mapped_head`). -/
 @[simp, grind =]
-theorem apply_subs_for_mapped_head_eq (trg : PreTrigger sig) (i : Fin trg.mapped_head.length) :
-    (trg.subs_for_mapped_head i).apply_function_free_conj (trg.rule.head[i.val]'(by rw [← length_mapped_head]; exact i.isLt)) =
-    trg.mapped_head[i.val] := by
+theorem apply_subs_for_mapped_head_eq (trg : PreTrigger sig) (i : Nat) (lt : i < trg.rule.head.length) :
+    (trg.subs_for_mapped_head i lt).apply_function_free_conj trg.rule.head[i] = trg.mapped_head[i]'(by grind) := by
   unfold mapped_head
   unfold GroundSubstitution.apply_function_free_conj
   unfold TermMapping.apply_generalized_atom_list
-  rw [List.getElem_map, List.getElem_zipIdx, List.map_inj_left, Nat.zero_add]
+  simp only [List.getElem_map, List.getElem_attach, List.getElem_zipIdx, List.map_inj_left, Nat.zero_add]
   intros
-  apply apply_subs_for_atom_eq trg i
+  apply apply_subs_for_atom_eq trg i lt
 
 /-- The list of fresh terms are the function terms introduced for the existential variables. -/
 @[expose]
 def fresh_terms_for_head_disjunct (trg : PreTrigger sig) (i : Nat) (lt : i < trg.rule.head.length) : List (GroundTerm sig) :=
-  (trg.rule.existential_vars_for_head_disjunct i lt).map (trg.functional_term_for_var i)
+  (trg.rule.existential_vars_for_head_disjunct i lt).attach.map (fun v => trg.functional_term_for_var i lt v.val v.property)
+
+/-- The functional term produces by an existential variable is one of the fresh terms. -/
+theorem mem_fresh_terms_of_functional_for_exis_var {trg : PreTrigger sig} {i : Nat} {lt : i < trg.rule.head.length} {v : sig.V}
+    (v_mem : v ∈ trg.rule.existential_vars_for_head_disjunct i lt) : trg.functional_term_for_var i lt v v_mem ∈ trg.fresh_terms_for_head_disjunct i lt := by
+  unfold fresh_terms_for_head_disjunct; rw [List.map_attach_eq_pmap]; apply List.mem_pmap_of_mem; exact v_mem
 
 /-- This theorem unfolds some of the internal definitions of `fresh_terms_for_head_disjunct`. -/
 theorem mem_fresh_terms {trg : PreTrigger sig} {i : Nat} {lt : i < trg.rule.head.length} :
-    ∀ t ∈ trg.fresh_terms_for_head_disjunct i lt, ∃ v ∈ trg.rule.existential_vars_for_head_disjunct i lt,
-    t = GroundTerm.func { ruleId := trg.rule.id, disjunctIndex := i, var := v, arity := trg.rule.frontier.length } (trg.rule.frontier.map trg.subs) (by rw [List.length_map]) := by
+    ∀ t ∈ trg.fresh_terms_for_head_disjunct i lt, ∃ (v : sig.V) (v_mem : v ∈ trg.rule.existential_vars_for_head_disjunct i lt),
+    t = GroundTerm.func { rule := trg.rule, headIdx := i, headIdx_lt := lt, v, v_mem } (trg.rule.frontier.map trg.subs) (by rw [List.length_map]; rfl) := by
   intro t t_mem
-  simp only [fresh_terms_for_head_disjunct, List.mem_map, functional_term_for_var] at t_mem
-  rcases t_mem with ⟨v, v_mem, t_mem⟩
-  exists v; exact ⟨v_mem, Eq.symm t_mem⟩
+  simp only [fresh_terms_for_head_disjunct, List.mem_map, functional_term_for_var, List.mem_attach] at t_mem
+  rcases t_mem with ⟨⟨v, v_mem⟩, _, t_mem⟩
+  exists v, v_mem; exact Eq.symm t_mem
 
 /-- Fresh terms are always functional. -/
 theorem term_functional_of_mem_fresh_terms {trg : PreTrigger sig} {i : Nat} {lt : i < trg.rule.head.length} :
@@ -250,19 +291,21 @@ theorem constant_not_mem_fresh_terms_for_head_disjunct {trg : PreTrigger sig} {i
 theorem frontier_term_not_mem_fresh_terms_for_head_disjunct {trg : PreTrigger sig} {i : Nat} {lt : i < trg.rule.head.length} :
     ∀ {t}, t ∈ trg.rule.frontier.map trg.subs -> ¬ t ∈ trg.fresh_terms_for_head_disjunct i lt := by
   intro t t_frontier t_fresh
-  simp only [fresh_terms_for_head_disjunct, List.mem_map] at t_fresh
-  rcases t_fresh with ⟨v, v_mem, t_fresh⟩; simp only [Rule.existential_vars_for_head_disjunct, List.mem_filter, decide_eq_true_eq] at v_mem
-  apply trg.result_term_not_in_frontier_image_of_var_not_in_frontier ⟨i, lt⟩ v v_mem.right
-  rw [apply_to_var_or_const_non_frontier_var _ _ _ v_mem.right]
+  simp only [fresh_terms_for_head_disjunct, List.mem_map, List.mem_attach] at t_fresh
+  rcases t_fresh with ⟨⟨v, v_mem⟩, _, t_fresh⟩
+  apply trg.result_term_not_in_frontier_image_of_var_existential i lt v v_mem
+  rw [apply_to_var_or_const_of_mem_existential_vars _ _ _ _ v_mem]
   rw [t_fresh]
   exact t_frontier
 
 /-- For a given fresh term, we can obtain the existential variable that introduced it. -/
 def existential_var_for_fresh_term (trg : PreTrigger sig) (i : Nat) (lt : i < trg.rule.head.length) (t : GroundTerm sig) (t_mem : t ∈ trg.fresh_terms_for_head_disjunct i lt) : sig.V :=
-  ((trg.rule.existential_vars_for_head_disjunct i lt).find? (fun v => trg.functional_term_for_var i v = t)).get (by
+  ((trg.rule.existential_vars_for_head_disjunct i lt).find? (fun v => (t.functionSymbol (term_functional_of_mem_fresh_terms _ t_mem)).v = v)).get (by
     simp only [List.find?_isSome, decide_eq_true_eq]
-    simp only [fresh_terms_for_head_disjunct, List.mem_map] at t_mem
-    exact t_mem)
+    simp only [fresh_terms_for_head_disjunct, List.mem_map, List.mem_attach] at t_mem
+    rcases t_mem with ⟨⟨v, v_mem⟩, _, t_mem⟩
+    exists v; constructor; exact v_mem
+    simp only [← t_mem, functional_term_for_var, GroundTerm.functionSymbol_func])
 
 /-- Indeed getting the existential variable for a functional term introduced for a variable yields exactly this variable (as expected). -/
 @[simp, grind =]
@@ -272,10 +315,12 @@ theorem existential_var_for_fresh_term_after_functional_term_for_var
     (lt : i < trg.rule.head.length)
     {v : sig.V}
     (v_mem : v ∈ trg.rule.existential_vars_for_head_disjunct i lt) :
-    trg.existential_var_for_fresh_term i lt (trg.functional_term_for_var i v) (List.mem_map_of_mem v_mem) = v := by
+    trg.existential_var_for_fresh_term i lt (trg.functional_term_for_var i lt v v_mem) (mem_fresh_terms_of_functional_for_exis_var v_mem) = v := by
   simp only [existential_var_for_fresh_term]
   apply Option.get_of_eq_some
-  simp only [List.find?_eq_some_iff_getElem, decide_eq_true_eq, true_and]
+  simp only [List.find?_eq_some_iff_getElem, decide_eq_true_eq]
+  constructor
+  . simp only [functional_term_for_var, GroundTerm.functionSymbol_func]
   let j := (trg.rule.existential_vars_for_head_disjunct i lt).idxOf v
   exists j, (List.idxOf_lt_length_of_mem v_mem)
   constructor
@@ -286,63 +331,62 @@ theorem existential_var_for_fresh_term_after_functional_term_for_var
     rcases k_lt with ⟨_, k_lt⟩
     specialize k_lt k (by simp)
     rw [beq_eq_false_iff_ne] at k_lt
-    rw [not_decide_eq_true, functional_term_for_var.injEq]
-    simp only [true_and]
-    exact k_lt
+    rw [not_decide_eq_true]
+    simp only [functional_term_for_var, GroundTerm.functionSymbol_func]
+    intro contra; apply k_lt; rw [contra]
 
 /-- For a fact in the trigger result, we can obtain the head atom that yields the fact. -/
-def atom_for_result_fact (trg : PreTrigger sig) {f : Fact sig} (i : Fin trg.mapped_head.length)
-    (f_mem : f ∈ trg.mapped_head[i.val]) : FunctionFreeAtom sig :=
-  let j := trg.mapped_head[i.val].idxOf f
-  let i' : Fin trg.rule.head.length := ⟨i.val, by rw [← length_mapped_head]; exact i.isLt⟩
-  let j' : Fin (trg.rule.head[i'.val].length) := ⟨j, by
-    have := trg.length_each_mapped_head i.val
-    rw [List.getElem?_eq_getElem i.isLt] at this
-    rw [List.getElem?_eq_getElem i'.isLt] at this
+def atom_for_result_fact (trg : PreTrigger sig) {f : Fact sig} (i : Nat) (lt : i < trg.rule.head.length)
+    (f_mem : f ∈ trg.mapped_head[i]'(by grind)) : FunctionFreeAtom sig :=
+  let j := (trg.mapped_head[i]'(by grind)).idxOf f
+  trg.rule.head[i][j]'(by
+    have := trg.length_each_mapped_head i
+    rw [List.getElem?_eq_getElem lt] at this
+    rw [List.getElem?_eq_getElem (by grind)] at this
     simp only [Option.map_some, Option.some_inj] at this
     rw [← this]
     apply List.idxOf_lt_length_of_mem
     exact f_mem
-  ⟩
-  trg.rule.head[i'.val][j'.val]
+  )
 
 /-- Applying the trigger on the atom from `atom_for_result_fact` indeed yields the correct fact. -/
 @[simp, grind =]
-theorem apply_on_atom_for_result_fact_is_fact (trg : PreTrigger sig) {f : Fact sig} (i : Fin trg.mapped_head.length)
-    (f_mem : f ∈ trg.mapped_head[i.val]) : trg.apply_to_function_free_atom i (trg.atom_for_result_fact i f_mem) = f := by
-  have : f = trg.mapped_head[i.val][trg.mapped_head[i.val].idxOf f]'(List.idxOf_lt_length_of_mem f_mem) := by rw [List.getElem_idxOf_of_mem]; exact f_mem
+theorem apply_on_atom_for_result_fact_is_fact (trg : PreTrigger sig) {f : Fact sig} (i : Nat) (lt : i < trg.rule.head.length)
+    (f_mem : f ∈ trg.mapped_head[i]'(by grind)) :
+    trg.apply_to_function_free_atom i lt (trg.atom_for_result_fact i lt f_mem) = f := by
+  have lt' : i < trg.mapped_head.length := by rw [length_mapped_head]; exact lt
+  have : f = trg.mapped_head[i][trg.mapped_head[i].idxOf f]'(List.idxOf_lt_length_of_mem f_mem) := by rw [List.getElem_idxOf_of_mem]; exact f_mem
   conv => right; rw [this]
   unfold atom_for_result_fact
   unfold mapped_head
   simp
 
 /-- The atom from `atom_for_result_fact` occurs in the correct rule head disjunct. -/
-theorem atom_for_result_fact_mem_head {trg : PreTrigger sig} {f : Fact sig} {i : Fin trg.mapped_head.length}
-    {f_mem : f ∈ trg.mapped_head[i.val]} : trg.atom_for_result_fact i f_mem ∈ trg.rule.head[i.val]'(by rw [← length_mapped_head]; exact i.isLt) := by
+theorem atom_for_result_fact_mem_head {trg : PreTrigger sig} {f : Fact sig} {i : Nat} {lt : i < trg.rule.head.length}
+    {f_mem : f ∈ trg.mapped_head[i]'(by grind)} : trg.atom_for_result_fact i lt f_mem ∈ trg.rule.head[i] := by
   simp [atom_for_result_fact]
 
 /-- For any term in the result (not just fresh ones), we can obtain the corresponding `VarOrConst` from the rule. -/
-def var_or_const_for_result_term (trg : PreTrigger sig) {f : Fact sig} {t : GroundTerm sig} (i : Fin trg.mapped_head.length)
-    (f_mem : f ∈ trg.mapped_head[i.val]) (t_mem : t ∈ f.terms) : VarOrConst sig :=
+def var_or_const_for_result_term (trg : PreTrigger sig) {f : Fact sig} {t : GroundTerm sig} (i : Nat) (lt : i < trg.rule.head.length)
+    (f_mem : f ∈ trg.mapped_head[i]'(by grind)) (t_mem : t ∈ f.terms) : VarOrConst sig :=
   let k := f.terms.idxOf t
-  let atom := trg.atom_for_result_fact i f_mem
-  let k' : Fin atom.terms.length := ⟨k, by
+  let atom := trg.atom_for_result_fact i lt f_mem
+  have lt' : k < atom.terms.length := by
     have isLt := List.idxOf_lt_length_of_mem t_mem
-    have := trg.apply_on_atom_for_result_fact_is_fact i f_mem
+    have := trg.apply_on_atom_for_result_fact_is_fact i lt f_mem
     conv at isLt => right; rw [← this]
     rw [TermMapping.length_terms_apply_generalized_atom] at isLt
     exact isLt
-  ⟩
-  atom.terms[k'.val]
+  atom.terms[k]
 
 /-- Applying the trigger on the `VarOrConst` from `var_or_const_for_result_term` indeed yields the correct term. -/
 @[simp, grind =]
 theorem apply_on_var_or_const_for_result_term_is_term (trg : PreTrigger sig) {f : Fact sig} {t : GroundTerm sig}
-    (i : Fin trg.mapped_head.length) (f_mem : f ∈ trg.mapped_head[i.val]) (t_mem : t ∈ f.terms) :
-    trg.apply_to_var_or_const i (trg.var_or_const_for_result_term i f_mem t_mem) = t := by
+    (i : Nat) (lt : i < trg.rule.head.length) (f_mem : f ∈ trg.mapped_head[i]'(by grind)) (t_mem : t ∈ f.terms) :
+    trg.apply_to_var_or_const i lt (trg.var_or_const_for_result_term i lt f_mem t_mem) = t := by
   have t_eq : t = f.terms[f.terms.idxOf t]'(List.idxOf_lt_length_of_mem t_mem) := by rw [List.getElem_idxOf_of_mem]; exact t_mem
-  have := trg.apply_on_atom_for_result_fact_is_fact i f_mem
-  have : (trg.apply_to_function_free_atom i (trg.atom_for_result_fact i f_mem)).terms = f.terms := by rw [this]
+  have := trg.apply_on_atom_for_result_fact_is_fact i lt f_mem
+  have : (trg.apply_to_function_free_atom i lt (trg.atom_for_result_fact i lt f_mem)).terms = f.terms := by rw [this]
   conv at t_eq => right; simp only [← this]
   conv at t_eq => right; left; simp only [this]
   conv => right; rw [t_eq]
@@ -353,70 +397,64 @@ theorem apply_on_var_or_const_for_result_term_is_term (trg : PreTrigger sig) {f 
 
 /-- For a term in a result fact, `var_or_const_for_result_term` returns a `VarOrConst` that is in `atom_for_result_fact`. -/
 theorem var_or_const_for_result_term_mem_atom_for_result_fact {trg : PreTrigger sig} {f : Fact sig} {t : GroundTerm sig}
-    {i : Fin trg.mapped_head.length} {f_mem : f ∈ trg.mapped_head[i.val]} {t_mem : t ∈ f.terms} :
-    trg.var_or_const_for_result_term i f_mem t_mem ∈ (trg.atom_for_result_fact i f_mem).terms := by
+    {i : Nat} {lt : i < trg.rule.head.length} {f_mem : f ∈ trg.mapped_head[i]'(by grind)} {t_mem : t ∈ f.terms} :
+    trg.var_or_const_for_result_term i lt f_mem t_mem ∈ (trg.atom_for_result_fact i lt f_mem).terms := by
   simp [var_or_const_for_result_term]
 
 /-- For a term in a result fact, `var_or_const_for_result_term` occurs in the correct head disjunct. -/
 theorem var_or_const_for_result_term_mem_terms_head {trg : PreTrigger sig} {f : Fact sig} {t : GroundTerm sig}
-    {i : Fin trg.mapped_head.length} {f_mem : f ∈ trg.mapped_head[i.val]} {t_mem : t ∈ f.terms} :
-    trg.var_or_const_for_result_term i f_mem t_mem ∈ (trg.rule.head[i.val]'(by rw [← length_mapped_head]; exact i.isLt)).terms := by
+    {i : Nat} {lt : i < trg.rule.head.length} {f_mem : f ∈ trg.mapped_head[i]'(by grind)} {t_mem : t ∈ f.terms} :
+    trg.var_or_const_for_result_term i lt f_mem t_mem ∈ trg.rule.head[i].terms := by
   unfold FunctionFreeConjunction.terms; apply List.mem_flatMap_of_mem; apply atom_for_result_fact_mem_head; exact f_mem; apply var_or_const_for_result_term_mem_atom_for_result_fact
 
 /-- A term occurs in the trigger result for a given head index if and only if one of the following three cases holds. 1. The term is a constant in the head. 2. The term results from mapping a frontier variable in the head. 3. The term is a fresh term of the head. -/
-theorem mem_terms_mapped_head_iff (trg : PreTrigger sig) (i : Nat) (lt : i < trg.mapped_head.length) :
-    ∀ t, t ∈ trg.mapped_head[i].flatMap GeneralizedAtom.terms ↔ (∃ c, c ∈ (trg.rule.head[i]'(by rw [← length_mapped_head]; exact lt)).consts ∧ GroundTerm.const c = t) ∨ t ∈ (trg.rule.frontier_for_head i (by rw [← length_mapped_head]; exact lt)).map trg.subs ∨ t ∈ trg.fresh_terms_for_head_disjunct i (by rw [← length_mapped_head]; exact lt) := by
+theorem mem_terms_mapped_head_iff (trg : PreTrigger sig) (i : Nat) (lt : i < trg.rule.head.length) :
+    ∀ t, t ∈ (trg.mapped_head[i]'(by grind)).flatMap GeneralizedAtom.terms ↔ (∃ c, c ∈ trg.rule.head[i].consts ∧ GroundTerm.const c = t) ∨ t ∈ (trg.rule.frontier_for_head i lt).map trg.subs ∨ t ∈ trg.fresh_terms_for_head_disjunct i lt := by
   intro t
   rw [List.mem_flatMap, List.mem_map]
   constructor
   . rintro ⟨f, f_mem, t_mem⟩
-    cases eq : trg.var_or_const_for_result_term ⟨i, lt⟩ f_mem t_mem with
+    cases eq : trg.var_or_const_for_result_term i lt f_mem t_mem with
     | const c =>
       apply Or.inl
       exists c
       constructor
       . rw [FunctionFreeConjunction.mem_consts]
-        exists trg.atom_for_result_fact ⟨i, lt⟩ f_mem
+        exists trg.atom_for_result_fact i lt f_mem
         constructor
         . apply atom_for_result_fact_mem_head
         . rw [← eq]
           apply var_or_const_for_result_term_mem_atom_for_result_fact
-      . rw [← trg.apply_on_var_or_const_for_result_term_is_term ⟨i, lt⟩ f_mem t_mem, eq]; rfl
+      . rw [← trg.apply_on_var_or_const_for_result_term_is_term i lt f_mem t_mem, eq]; rfl
     | var v =>
       apply Or.inr
-      cases Decidable.em (v ∈ trg.rule.frontier) with
-      | inl v_mem_frontier =>
-        have v_mem_frontier : v ∈ trg.rule.frontier_for_head i (by rw [← length_mapped_head]; exact lt) := by
-          apply Rule.mem_frontier_for_head_of_mem_frontier_of_mem_head_terms
-          . exact v_mem_frontier
-          . rw [← eq]; apply var_or_const_for_result_term_mem_terms_head
-        apply Or.inl
-        exists v
-        constructor
-        . exact v_mem_frontier
-        . rw [← trg.apply_on_var_or_const_for_result_term_is_term ⟨i, lt⟩ f_mem t_mem, eq, apply_to_var_or_const_frontier_var]; rw [Rule.mem_frontier_iff_mem_frontier_for_head]; exists i, (by rw [← length_mapped_head]; exact lt)
-      | inr v_nmem_frontier =>
+      cases Decidable.em (v ∈ trg.rule.existential_vars_for_head_disjunct i lt) with
+      | inl v_exis =>
         apply Or.inr
-        unfold fresh_terms_for_head_disjunct Rule.existential_vars_for_head_disjunct
-        simp only [List.mem_map, List.mem_filter, decide_eq_true_iff, FunctionFreeConjunction.mem_vars]
-        exists v
-        constructor
-        constructor
-        . exists trg.atom_for_result_fact ⟨i, lt⟩ f_mem
-          constructor
-          . apply atom_for_result_fact_mem_head
-          . rw [← eq]
-            apply var_or_const_for_result_term_mem_atom_for_result_fact
-        . exact v_nmem_frontier
-        . rw [← trg.apply_on_var_or_const_for_result_term_is_term ⟨i, lt⟩ f_mem t_mem, eq, apply_to_var_or_const_non_frontier_var]; exact v_nmem_frontier
+        rw [← trg.apply_on_var_or_const_for_result_term_is_term i lt f_mem t_mem, eq]
+        rw [trg.apply_to_var_or_const_of_mem_existential_vars _ _ _ v_exis]
+        apply trg.mem_fresh_terms_of_functional_for_exis_var
+      | inr v_not_exis =>
+        apply Or.inl
+        rw [← trg.apply_on_var_or_const_for_result_term_is_term i lt f_mem t_mem, eq]
+        exists v; constructor
+        . have v_mem_head : v ∈ trg.rule.head[i].vars := by
+            rw [FunctionFreeConjunction.mem_vars', ← eq]
+            apply var_or_const_for_result_term_mem_terms_head
+          apply trg.rule.mem_frontier_for_head_of_mem_frontier_of_mem_head_terms _ _ (by rw [← FunctionFreeConjunction.mem_vars']; exact v_mem_head)
+          unfold Rule.existential_vars_for_head_disjunct at v_not_exis
+          rw [List.mem_filter, not_and, decide_not, not_decide_eq_true, Decidable.not_not] at v_not_exis
+          apply v_not_exis
+          exact v_mem_head
+        . rw [apply_to_var_or_const_of_not_mem_existential_vars _ _ _ _ v_not_exis]
   . intro h
     cases h with
     | inl h =>
       rcases h with ⟨c, c_mem, t_eq⟩
       rcases FunctionFreeConjunction.mem_consts.mp c_mem with ⟨a, a_mem, c_mem⟩
-      exists trg.apply_to_function_free_atom i a
+      exists trg.apply_to_function_free_atom i lt a
       constructor
-      . unfold mapped_head; simp only [List.getElem_map, List.getElem_zipIdx, Nat.zero_add]; apply List.mem_map_of_mem; exact a_mem
+      . unfold mapped_head; grind
       . simp only [apply_to_function_free_atom, TermMapping.apply_generalized_atom]
         rw [List.mem_map]
         exists .const c
@@ -425,39 +463,41 @@ theorem mem_terms_mapped_head_iff (trg : PreTrigger sig) (i : Nat) (lt : i < trg
     | inl h =>
       rcases h with ⟨v, v_mem, t_eq⟩
       rcases FunctionFreeConjunction.mem_vars.mp (trg.rule.frontier_for_head_subset_vars_head _ v_mem) with ⟨a, a_mem, v_mem'⟩
-      exists trg.apply_to_function_free_atom i a
+      exists trg.apply_to_function_free_atom i lt a
       constructor
-      . unfold mapped_head; simp only [List.getElem_map, List.getElem_zipIdx, Nat.zero_add]; apply List.mem_map_of_mem; exact a_mem
+      . unfold mapped_head; grind
       . simp only [apply_to_function_free_atom, TermMapping.apply_generalized_atom]
         rw [List.mem_map]
         exists .var v
         constructor
         . exact v_mem'
-        . rw [apply_to_var_or_const_frontier_var _ _ _ (by apply Rule.mem_frontier_iff_mem_frontier_for_head.mpr; exists i, (by rw [← length_mapped_head]; exact lt))]; exact t_eq
+        . rw [apply_to_var_or_const_frontier_var _ _ _ _ (by apply Rule.mem_frontier_iff_mem_frontier_for_head.mpr; exists i, lt)]; exact t_eq
     | inr h =>
-      unfold fresh_terms_for_head_disjunct Rule.existential_vars_for_head_disjunct at h
-      simp only [List.mem_map, List.mem_filter, decide_eq_true_iff, FunctionFreeConjunction.mem_vars] at h
-      rcases h with ⟨v, ⟨⟨a, a_mem, v_mem⟩, v_not_frontier⟩, t_eq⟩
-      exists trg.apply_to_function_free_atom i a
+      unfold fresh_terms_for_head_disjunct at h
+      simp only [List.mem_map, List.mem_attach] at h
+      rcases h with ⟨⟨v, v_mem⟩, _, t_eq⟩
+      have v_mem_head := trg.rule.mem_head_vars_of_mem_existential_vars_for_head_disjunct _ v_mem
+      rw [FunctionFreeConjunction.mem_vars] at v_mem_head; rcases v_mem_head with ⟨a, a_mem, v_mem_a⟩
+      exists trg.apply_to_function_free_atom i lt a
       constructor
-      . unfold mapped_head; simp only [List.getElem_map, List.getElem_zipIdx, Nat.zero_add]; apply List.mem_map_of_mem; exact a_mem
+      . unfold mapped_head; grind
       . simp only [apply_to_function_free_atom, TermMapping.apply_generalized_atom]
         rw [List.mem_map]
         exists .var v
         constructor
-        . exact v_mem
-        . rw [apply_to_var_or_const_non_frontier_var _ _ _ v_not_frontier]; exact t_eq
+        . exact v_mem_a
+        . rw [apply_to_var_or_const_of_mem_existential_vars _ _ _ _ v_mem]; exact t_eq
 
 /-- The constants in the trigger result are a subset of the constants from the mapped frontier terms and the constants that occur directly in the rule head. -/
-theorem mapped_head_constants_subset (trg : PreTrigger sig) (i : Fin trg.mapped_head.length) :
-    FactSet.constants trg.mapped_head[i.val].toSet ⊆ (((trg.rule.frontier.map (trg.subs_for_mapped_head i)).flatMap GroundTerm.constants) ++ (trg.rule.head[i.val]'(by rw [← length_mapped_head]; exact i.isLt)).consts).toSet := by
+theorem mapped_head_constants_subset (trg : PreTrigger sig) (i : Nat) (lt : i < trg.rule.head.length) :
+    FactSet.constants (trg.mapped_head[i]'(by grind)).toSet ⊆ (((trg.rule.frontier.map (trg.subs_for_mapped_head i lt)).flatMap GroundTerm.constants) ++ trg.rule.head[i].consts).toSet := by
   intro c c_mem
   rw [List.mem_toSet, List.mem_append]
   rw [FactSet.mem_constants_toSet, List.mem_flatMap] at c_mem
   rcases c_mem with ⟨f, f_mem, c_mem⟩
   simp only [Fact.constants, List.mem_flatMap] at c_mem
   rcases c_mem with ⟨t, t_mem, c_mem⟩
-  have t_mem : t ∈ trg.mapped_head[i.val].flatMap GeneralizedAtom.terms := by rw [List.mem_flatMap]; exists f
+  have t_mem : t ∈ (trg.mapped_head[i]'(by grind)).flatMap GeneralizedAtom.terms := by rw [List.mem_flatMap]; exists f
   rw [mem_terms_mapped_head_iff] at t_mem
   cases t_mem with
   | inl t_mem =>
@@ -492,8 +532,8 @@ theorem mapped_head_constants_subset (trg : PreTrigger sig) (i : Fin trg.mapped_
 
 /-- The trigger is loaded for a `FactSet` if its mapped body occurs in the fact set. -/
 @[expose]
-def loaded (trg : PreTrigger sig) (F : FactSet sig) : Prop :=
-  trg.mapped_body.toSet ⊆ F
+def loaded (trg : PreTrigger sig) (fs : FactSet sig) : Prop :=
+  trg.mapped_body.toSet ⊆ fs
 
 /-- Applying a `GroundTermMapping` that is the id on constants after the trigger substitution and on the fact set preserves loadedness. -/
 theorem term_mapping_preserves_loadedness (trg : PreTrigger sig) (fs : FactSet sig) (h : GroundTermMapping sig) (h_id : h.isIdOnConstants) :
@@ -515,35 +555,33 @@ theorem term_mapping_preserves_loadedness (trg : PreTrigger sig) (fs : FactSet s
 
 /-- A trigger head is satisfied for a `FactSet` if there exists a substitution that agrees with the trigger substitution on all frontier variable such that the mapping of the head occurs in the fact set. This corresponds to FOL semantics. It is **important** to note here that a trigger being satisfied in this sense does not necessarily mean that it is obsolete! Obsolescence might be defined almost arbitrarily and for example in the Skolem chase, a satisfied trigger is often not obsolete. However, for the restricted (aka. standard) chase, obsolescence is defined via satisfaction. -/
 @[expose]
-def satisfied_for_disj (trg : PreTrigger sig) (fs : FactSet sig) (disj_index : Fin trg.rule.head.length) : Prop :=
+def satisfied_for_disj (trg : PreTrigger sig) (fs : FactSet sig) (i : Nat) (lt : i < trg.rule.head.length) : Prop :=
   ∃ (s : GroundSubstitution sig),
     (∀ v, v ∈ (Rule.frontier trg.rule) → s v = trg.subs v) ∧
-    ((s.apply_function_free_conj (trg.rule.head[disj_index.val])).toSet ⊆ fs)
+    ((s.apply_function_free_conj (trg.rule.head[i])).toSet ⊆ fs)
 
 /-- If the exact trigger result is contained in the fact set, then the trigger is also satisfied. -/
 theorem satisfied_for_disj_of_mapped_head_contained (trg : PreTrigger sig) (fs : FactSet sig)
-    (disj_index : Fin trg.rule.head.length) :
-    (trg.mapped_head[disj_index.val]'(by rw [length_mapped_head]; exact disj_index.isLt)).toSet ⊆ fs ->
-    trg.satisfied_for_disj fs disj_index := by
+    (i : Nat) (lt : i < trg.rule.head.length) :
+    (trg.mapped_head[i]'(by grind)).toSet ⊆ fs ->
+    trg.satisfied_for_disj fs i lt := by
   intro h
-  let i : Fin trg.mapped_head.length := ⟨disj_index.val, by rw [length_mapped_head]; exact disj_index.isLt⟩
-  exists trg.subs_for_mapped_head i
+  exists trg.subs_for_mapped_head i lt
   constructor
-  . intro v v_mem; unfold subs_for_mapped_head; rw [trg.apply_to_var_or_const_frontier_var i v v_mem]
-  . rw [trg.apply_subs_for_mapped_head_eq i]; exact h
+  . intro v v_mem; unfold subs_for_mapped_head; rw [trg.apply_to_var_or_const_frontier_var _ _ _ v_mem]
+  . rw [trg.apply_subs_for_mapped_head_eq i lt]; exact h
 
 /-- The trigger is satisfied if it is satisfied for some head. Note that this checks out with FOL semantics since the heads are part of a big disjunction. -/
 @[expose]
-def satisfied (trg : PreTrigger sig) (F : FactSet sig) : Prop :=
-  ∃ disj_index, trg.satisfied_for_disj F disj_index
+def satisfied (trg : PreTrigger sig) (fs : FactSet sig) : Prop :=
+  ∃ i lt, trg.satisfied_for_disj fs i lt
 
 /-- If a trigger is satisfied, then it is also satisfied on all supersets. -/
 theorem satisfied_of_satisfied_subset {trg : PreTrigger sig} {fs fs2 : FactSet sig} (sub : fs ⊆ fs2) :
     trg.satisfied fs -> trg.satisfied fs2 := by
   simp [PreTrigger.satisfied, PreTrigger.satisfied_for_disj]
-  intro i subs frontier_same_under_subs applied_head_sub_fs
-  exists i
-  exists subs
+  intro i lt subs frontier_same_under_subs applied_head_sub_fs
+  exists i, lt, subs
   constructor
   . apply frontier_same_under_subs
   . apply Set.subset_trans
@@ -622,54 +660,62 @@ theorem mapped_body_eq_of_strong_equiv {trg1 trg2 : PreTrigger sig} : trg1.stron
   . rw [equiv.left]; exact a_mem
 
 /-- Applying two equivalent triggers to the same (head) atom yields the same result. -/
-theorem apply_to_function_free_atom_eq_of_equiv {trg1 trg2 : PreTrigger sig} :
-    trg1.equiv trg2 -> ∀ (i : Nat), ∀ a, trg1.apply_to_function_free_atom i a = trg2.apply_to_function_free_atom i a := by
-  unfold equiv
-  intro h i a
+theorem apply_to_function_free_atom_eq_of_equiv {trg1 trg2 : PreTrigger sig} (equiv : trg1.equiv trg2) :
+    ∀ (i : Nat), (lt : i < trg1.rule.head.length) ->
+    ∀ a ∈ trg1.rule.head[i], trg1.apply_to_function_free_atom i lt a = trg2.apply_to_function_free_atom i (by rw [← equiv.left]; exact lt) a := by
+  intro i lt a a_mem
   apply TermMapping.apply_generalized_atom_congr_left
   intro voc voc_mem
   cases voc with
   | const c => simp
   | var v =>
-    cases Decidable.em (v ∈ trg1.rule.frontier) with
-    | inl v_front =>
-      have v_front_2 : v ∈ trg2.rule.frontier := by rw [← h.left]; exact v_front
-      rw [PreTrigger.apply_to_var_or_const_frontier_var _ _ _ v_front]
-      rw [PreTrigger.apply_to_var_or_const_frontier_var _ _ _ v_front_2]
-      apply h.right
-      exact v_front
-    | inr v_front =>
-      have v_front_2 : ¬ v ∈ trg2.rule.frontier := by rw [← h.left]; exact v_front
-      rw [PreTrigger.apply_to_var_or_const_non_frontier_var _ _ _ v_front]
-      rw [PreTrigger.apply_to_var_or_const_non_frontier_var _ _ _ v_front_2]
+    cases Decidable.em (v ∈ trg1.rule.existential_vars_for_head_disjunct i lt) with
+    | inl v_exis =>
+      rw [trg1.apply_to_var_or_const_of_mem_existential_vars _ _ _ v_exis]
+      simp only [equiv.left] at v_exis
+      rw [trg2.apply_to_var_or_const_of_mem_existential_vars _ _ _ v_exis]
       unfold PreTrigger.functional_term_for_var
-      simp only [← h.left]
+      simp only [← equiv.left]
       have : trg1.rule.frontier.map trg1.subs = trg1.rule.frontier.map trg2.subs := by
         rw [List.map_inj_left]
-        exact h.right
+        exact equiv.right
       simp only [this]
+    | inr v_not_exis =>
+      have v_front : v ∈ trg2.rule.frontier := by
+        rw [← equiv.left]
+        unfold Rule.existential_vars_for_head_disjunct at v_not_exis
+        rw [List.mem_filter, not_and, decide_not, not_decide_eq_true, Decidable.not_not] at v_not_exis
+        apply v_not_exis
+        rw [FunctionFreeConjunction.mem_vars]
+        exists a
+      rw [trg2.apply_to_var_or_const_frontier_var _ _ _ v_front]
+      simp only [← equiv.left] at v_front
+      rw [trg1.apply_to_var_or_const_frontier_var _ _ _ v_front]
+      apply equiv.right
+      exact v_front
 
 /-- As intended, equivalent triggers have the same result. -/
 @[grind ->]
 theorem result_eq_of_equiv {trg1 trg2 : PreTrigger sig} : trg1.equiv trg2 -> trg1.mapped_head = trg2.mapped_head := by
-  unfold equiv
-  intro h
+  intro equiv
   unfold mapped_head
-  rw [h.left]
-  rw [List.map_inj_left]
-  intro e e_mem
+  simp only [List.map_attach_eq_pmap]
+  simp only [equiv.left]
+  apply List.pmap_congr_left
+  intro pair _ pair_mem1 pair_mem2
   rw [List.map_inj_left]
   intro a a_mem
   apply apply_to_function_free_atom_eq_of_equiv
-  exact h
+  . exact equiv
+  . rw [← (List.mem_zipIdx' pair_mem1).right]; exact a_mem
 
 /-- Equivalent triggers are satisfied on the same fact sets. -/
 theorem satisfied_preserved_of_equiv {trg1 trg2 : PreTrigger sig} : trg1.equiv trg2 -> ∀ {fs}, trg1.satisfied fs ↔ trg2.satisfied fs := by
   intro equiv fs
   constructor
   . intro h
-    rcases h with ⟨i, s, front, subset⟩
-    exists ⟨i, by rw [← equiv.left]; exact i.isLt⟩, s
+    rcases h with ⟨i, lt, s, front, subset⟩
+    exists i, by rw [← equiv.left]; exact lt, s
     constructor
     . intro v v_mem
       rw [← equiv.right]
@@ -677,14 +723,43 @@ theorem satisfied_preserved_of_equiv {trg1 trg2 : PreTrigger sig} : trg1.equiv t
       . rw [equiv.left]; exact v_mem
     . simp only [← equiv.left]; exact subset
   . intro h
-    rcases h with ⟨i, s, front, subset⟩
-    exists ⟨i, by rw [equiv.left]; exact i.isLt⟩, s
+    rcases h with ⟨i, lt, s, front, subset⟩
+    exists i, by rw [equiv.left]; exact lt, s
     constructor
     . intro v v_mem
       rw [equiv.right]
       . apply front; rw [← equiv.left]; exact v_mem
       . exact v_mem
     . simp only [equiv.left]; exact subset
+
+/-- If a ground term is fresh in two `PreTrigger`s for two head indices, then actually these two `PreTrigger`s (and indices) need to be equivalent (the same)! Why is this the case? Fresh terms are always Skolem function terms. Therefore they contain a rule, which needs to be the same for both triggers. The head indices are also part of the functional term so a similar argument can be made to show that these need to be equal. To see why the triggers also need to agree on their frontier mapping, we only need to remind ourselves that the Skolem term contains all the mapped frontier terms as arguments. -/
+theorem equiv_of_term_mem_fresh_terms_for_head_disjunct
+    {trg1 trg2 : PreTrigger sig}
+    {i1 i2 : Nat}
+    {lt1 : i1 < trg1.rule.head.length}
+    {lt2 : i2 < trg2.rule.head.length}
+    {t : GroundTerm sig} :
+    (t ∈ trg1.fresh_terms_for_head_disjunct i1 lt1) ->
+      (t ∈ trg2.fresh_terms_for_head_disjunct i2 lt2) ->
+        trg1.equiv trg2 ∧ i1 = i2 := by
+  unfold PreTrigger.fresh_terms_for_head_disjunct PreTrigger.functional_term_for_var
+  simp only [List.mem_map]
+  rintro ⟨v1, v1_mem, t_eq⟩ ⟨v2, v2_mem, t_eq2⟩
+  rw [← t_eq2] at t_eq
+  rw [GroundTerm.func.injEq, SkolemFS.mk.injEq] at t_eq
+  have rules_eq : trg1.rule = trg2.rule := t_eq.left.left
+  constructor
+  . unfold equiv
+    constructor
+    . exact rules_eq
+    . have right := t_eq.right
+      have : trg1.rule.frontier = trg2.rule.frontier := by rw [rules_eq]
+      rw [← this] at right
+      rw [List.map_eq_map_iff] at right
+      intro v v_mem
+      apply right
+      exact v_mem
+  . exact t_eq.left.right.left
 
 end PreTrigger
 
