ExistentialRules/ChaseSequence/Termination/ConstantMappings/InterplayWithBacktracking/BacktrackingUnderConstantMappingSubsetOfComposingWithSubs/PreTrigger.lean
@@ -17,25 +17,56 @@ public section
 
 variable {sig : Signature} [DecidableEq sig.C] [DecidableEq sig.V] [DecidableEq sig.P]
 
+/--
+The affected rules for triggers with the `PreTrigger.same_skeleton` are the same.
+-/
+theorem PreTrigger.affected_rules_eq_of_same_skeleton {trg trg2 : PreTrigger sig} (same_skeleton : trg.same_skeleton trg2) :
+    trg.affected_rules_for_backtracking = trg2.affected_rules_for_backtracking := by
+  unfold affected_rules_for_backtracking
+  rw [List.cons_eq_cons]; constructor; exact same_skeleton.left
+  simp only [List.flatMap_def, List.map_flatten]
+  apply List.flatten_eq_of_eq; apply List.flatten_eq_of_eq
+  apply List.ext_getElem
+  . simp [same_skeleton.left]
+  . intro i _ _
+    simp only [List.getElem_map, PreTrigger.mapped_body, GroundSubstitution.apply_function_free_conj, TermMapping.apply_generalized_atom_list]
+    simp only [TermMapping.apply_generalized_atom]
+    apply List.ext_getElem
+    . simp [same_skeleton.left]
+    . intro j _ _
+      simp only [List.getElem_map]
+      apply GroundTerm.rules_eq_of_same_skeleton
+      simp only [← same_skeleton.left]
+      cases eq : (trg.rule.body[i]'(by grind)).terms[j]'(by grind) with
+      | const c => simp only [GroundSubstitution.apply_var_or_const]; exact GroundTerm.same_skeleton_const
+      | var v =>
+        apply GroundSubstitution.same_skeleton_of_mem_vars same_skeleton.right
+        rw [List.mem_eraseDupsKeepRight, FunctionFreeConjunction.mem_vars', ← eq]
+        apply List.mem_flatMap_of_mem
+        . exact List.getElem_mem (n := i) (by grind)
+        . simp
+
+/--
+Since a strict constant mapping does not change term structure, the affected rules of a trigger stay the same when a strict constant mapping is applied after the substitution.
+-/
+theorem PreTrigger.affected_rules_eq_of_composing_with_subs {trg : PreTrigger sig} : ∀ (g : StrictConstantMapping sig),
+    trg.affected_rules_for_backtracking = { rule := trg.rule, subs := g.toConstantMapping.apply_ground_term ∘ trg.subs : PreTrigger sig}.affected_rules_for_backtracking := by
+  intro g
+  apply affected_rules_eq_of_same_skeleton
+  apply same_skeleton_under_strict_constant_mapping
+
 theorem PreTrigger.backtracking_under_constant_mapping_subset_of_composing_with_subs
     [GetFreshInhabitant sig.C]
     [Inhabited sig.C]
-    (rl : RuleList sig)
-    (trg : PreTrigger sig)
-    (trg_ruleIds_valid : trg.skolem_ruleIds_valid rl)
-    (trg_disjIdx_valid : trg.skolem_disjIdx_valid rl trg_ruleIds_valid)
-    (trg_rule_arity_valid : trg.skolem_rule_arity_valid rl trg_ruleIds_valid)
-    (trg_rule_in_rl : trg.rule ∈ rl.rules) :
-    let backtracking := trg.backtrackFacts rl trg_ruleIds_valid trg_disjIdx_valid trg_rule_arity_valid
-    ∀ (g : StrictConstantMapping sig), (∀ d, (d ∈ rl.rules.flatMap Rule.constants) -> g d = d) ->
+    (trg : PreTrigger sig) :
+    ∀ (g : StrictConstantMapping sig), (∀ d ∈ trg.affected_rules_for_backtracking.flatMap Rule.constants, g d = d) ->
       ∃ (fresh_constant_remapping : StrictConstantMapping sig),
-      (∀ d ∉ backtracking.snd, fresh_constant_remapping d = d) ∧
-      ((StrictConstantMapping.toConstantMapping (fun c => if c ∈ backtracking.snd then fresh_constant_remapping c else g c)).apply_fact_set backtracking.fst.toSet ⊆
-      ({rule := trg.rule, subs := g.toConstantMapping.apply_ground_term ∘ trg.subs : PreTrigger sig}.backtrackFacts rl (trg.compose_strict_constant_mapping_preserves_ruleId_validity g rl trg_ruleIds_valid) (trg.compose_strict_constant_mapping_preserves_disjIdx_validity g rl trg_ruleIds_valid trg_disjIdx_valid) (trg.compose_strict_constant_mapping_preserves_rule_arity_validity g rl trg_ruleIds_valid trg_rule_arity_valid)).fst.toSet) ∧
-      (backtracking.snd.map fresh_constant_remapping = ({rule := trg.rule, subs := g.toConstantMapping.apply_ground_term ∘ trg.subs : PreTrigger sig}.backtrackFacts rl (trg.compose_strict_constant_mapping_preserves_ruleId_validity g rl trg_ruleIds_valid) (trg.compose_strict_constant_mapping_preserves_disjIdx_validity g rl trg_ruleIds_valid trg_disjIdx_valid) (trg.compose_strict_constant_mapping_preserves_rule_arity_validity g rl trg_ruleIds_valid trg_rule_arity_valid)).snd) := by
-  intro backtracking g g_id
-  let forbidden_constants := trg.mapped_body.flatMap Fact.constants ++ rl.rules.flatMap Rule.constants
-  rcases GroundTerm.backtrackFacts_list_under_constant_mapping_subset_of_composing_with_subs rl (trg.mapped_body.flatMap GeneralizedAtom.terms) trg_ruleIds_valid trg_disjIdx_valid trg_rule_arity_valid forbidden_constants (by apply List.subset_append_of_subset_left; intro d d_mem; rw [List.mem_flatMap] at d_mem; rcases d_mem with ⟨t, t_mem, d_mem⟩; rw [List.mem_flatMap] at t_mem; rcases t_mem with ⟨f, f_mem, t_mem⟩; rw [List.mem_flatMap]; exists f; constructor; exact f_mem; unfold Fact.constants; rw [List.mem_flatMap]; exists t) (by apply List.subset_append_of_subset_right; simp) g g_id with ⟨fresh_constant_remapping, fresh_constant_remapping_h⟩
+      (∀ d ∉ trg.backtrackFacts.snd, fresh_constant_remapping d = d) ∧
+      ((StrictConstantMapping.toConstantMapping (fun c => if c ∈ trg.backtrackFacts.snd then fresh_constant_remapping c else g c)).apply_fact_set trg.backtrackFacts.fst.toSet ⊆
+      {rule := trg.rule, subs := g.toConstantMapping.apply_ground_term ∘ trg.subs : PreTrigger sig}.backtrackFacts.fst.toSet) ∧
+      (trg.backtrackFacts.snd.map fresh_constant_remapping = {rule := trg.rule, subs := g.toConstantMapping.apply_ground_term ∘ trg.subs : PreTrigger sig}.backtrackFacts.snd) := by
+  intro g g_id
+  rcases GroundTerm.backtrackFacts_list_under_constant_mapping_subset_of_composing_with_subs (trg.mapped_body.flatMap GeneralizedAtom.terms) trg.initial_forbidden_constants_for_backtracking (by apply List.subset_append_of_subset_left; intro d d_mem; rw [List.mem_flatMap] at d_mem; rcases d_mem with ⟨t, t_mem, d_mem⟩; rw [List.mem_flatMap] at t_mem; rcases t_mem with ⟨f, f_mem, t_mem⟩; rw [List.mem_flatMap]; exists f; constructor; exact f_mem; unfold Fact.constants; rw [List.mem_flatMap]; exists t) (by apply List.subset_append_of_subset_right; simp [PreTrigger.affected_rules_for_backtracking]) g (by intro d d_mem; apply g_id; apply List.mem_append_right; exact d_mem) with ⟨fresh_constant_remapping, fresh_constant_remapping_h⟩
 
   have mapped_body_map_swap : (trg.mapped_body.flatMap GeneralizedAtom.terms).map g.toConstantMapping.apply_ground_term = { rule := trg.rule, subs := g.toConstantMapping.apply_ground_term ∘ trg.subs : PreTrigger sig }.mapped_body.flatMap GeneralizedAtom.terms := by
     rw [List.map_flatMap]
@@ -54,25 +85,22 @@ theorem PreTrigger.backtracking_under_constant_mapping_subset_of_composing_with_
       rw [ConstantMapping.apply_ground_term_constant]
       simp only [StrictConstantMapping.toConstantMapping, Function.comp_apply, GroundTerm.const, Subtype.mk.injEq, FiniteTree.leaf.injEq]
       apply g_id
+      apply List.mem_append_left
+      unfold Rule.constants
+      rw [List.mem_append]
+      apply Or.inl
+      unfold FunctionFreeConjunction.consts
       rw [List.mem_flatMap]
-      exists trg.rule
+      exists a
       constructor
-      . exact trg_rule_in_rl
-      . unfold Rule.constants
-        rw [List.mem_append]
-        apply Or.inl
-        unfold FunctionFreeConjunction.consts
-        rw [List.mem_flatMap]
-        exists a
-        constructor
-        . exact a_mem
-        . unfold FunctionFreeAtom.constants
-          apply VarOrConst.mem_filterConsts_of_const
-          exact voc_mem
+      . exact a_mem
+      . unfold FunctionFreeAtom.constants
+        apply VarOrConst.mem_filterConsts_of_const
+        exact voc_mem
     | var v => rfl
 
-  have forbidden_constants_map_g_eq : forbidden_constants.map g = ({ rule := trg.rule, subs := g.toConstantMapping.apply_ground_term ∘ trg.subs : PreTrigger sig }.mapped_body.flatMap Fact.constants) ++ rl.rules.flatMap Rule.constants := by
-    unfold forbidden_constants
+  have forbidden_constants_map_g_eq : trg.initial_forbidden_constants_for_backtracking.map g = { rule := trg.rule, subs := g.toConstantMapping.apply_ground_term ∘ trg.subs : PreTrigger sig }.initial_forbidden_constants_for_backtracking := by
+    unfold PreTrigger.initial_forbidden_constants_for_backtracking
     rw [List.map_append]
     apply List.append_eq_append_of_parts_eq
     . rw [List.map_flatMap]
@@ -94,27 +122,25 @@ theorem PreTrigger.backtracking_under_constant_mapping_subset_of_composing_with_
         simp only [GroundTerm.const, FiniteTree.leaves]
         simp only [List.map_cons, List.map_nil, List.cons.injEq, and_true]
         apply g_id
+        apply List.mem_append_left
+        unfold Rule.constants
+        rw [List.mem_append]
+        apply Or.inl
+        unfold FunctionFreeConjunction.consts
         rw [List.mem_flatMap]
-        exists trg.rule
+        exists a
         constructor
-        . exact trg_rule_in_rl
-        . unfold Rule.constants
-          rw [List.mem_append]
-          apply Or.inl
-          unfold FunctionFreeConjunction.consts
-          rw [List.mem_flatMap]
-          exists a
-          constructor
-          . exact a_mem
-          . unfold FunctionFreeAtom.constants
-            apply VarOrConst.mem_filterConsts_of_const
-            exact voc_mem
+        . exact a_mem
+        . unfold FunctionFreeAtom.constants
+          apply VarOrConst.mem_filterConsts_of_const
+          exact voc_mem
       | var v =>
         simp only [ConstantMapping.apply_ground_term, ConstantMapping.apply_pre_ground_term]
         rw [StrictConstantMapping.map_leaves_eq_leaves_mapLeaves]
-    . apply List.map_id_of_id_on_all_mem
-      intro d d_mem
-      apply g_id
+    . rw [affected_rules_eq_of_composing_with_subs]
+      apply List.map_id_of_id_on_all_mem
+      intro d d_mem; apply g_id
+      rw [affected_rules_eq_of_composing_with_subs]
       exact d_mem
 
   exists fresh_constant_remapping
@@ -124,7 +150,7 @@ theorem PreTrigger.backtracking_under_constant_mapping_subset_of_composing_with_
   . intro e e_mem
     rw [GroundTermMapping.mem_applyFactSet] at e_mem
     rcases e_mem with ⟨f, f_mem, e_eq⟩
-    simp only [List.mem_toSet, backtracking, backtrackFacts, List.mem_append] at f_mem
+    simp only [List.mem_toSet, backtrackFacts, List.mem_append] at f_mem
     simp only [List.mem_toSet, backtrackFacts, List.mem_append]
     cases f_mem with
     | inl f_mem =>
@@ -140,11 +166,10 @@ theorem PreTrigger.backtracking_under_constant_mapping_subset_of_composing_with_
           rw [← ConstantMapping.apply_fact_eq_groundTermMapping_applyFact]
           apply ConstantMapping.apply_fact_congr_left
           intro d d_mem
-          have : d ∉ backtracking.snd := by
+          have : d ∉ trg.backtrackFacts.snd := by
             intro contra
             apply GroundTerm.backtrackFacts_list_fresh_constants_not_forbidden d contra
-            rw [List.mem_append]
-            apply Or.inl
+            apply List.mem_append_left
             rw [List.mem_flatMap]
             exists f
             constructor
@@ -157,16 +182,13 @@ theorem PreTrigger.backtracking_under_constant_mapping_subset_of_composing_with_
         . intro d d_mem
           simp only [ConstantMapping.apply_ground_term, ConstantMapping.apply_pre_ground_term, StrictConstantMapping.toConstantMapping, Function.comp_apply, GroundTerm.const, Subtype.mk.injEq, FiniteTree.mapLeaves, FiniteTree.leaf.injEq]
           apply g_id
+          apply List.mem_append_left
+          unfold Rule.constants
+          rw [List.mem_append]
+          apply Or.inl
+          unfold FunctionFreeConjunction.consts
           rw [List.mem_flatMap]
-          exists trg.rule
-          constructor
-          . exact trg_rule_in_rl
-          . unfold Rule.constants
-            rw [List.mem_append]
-            apply Or.inl
-            unfold FunctionFreeConjunction.consts
-            rw [List.mem_flatMap]
-            exists a
+          exists a
     | inr f_mem =>
       apply Or.inr
       simp only [mapped_body_map_swap] at fresh_constant_remapping_h
@@ -175,7 +197,7 @@ theorem PreTrigger.backtracking_under_constant_mapping_subset_of_composing_with_
       apply fresh_constant_remapping_h.right.left
       rw [GroundTermMapping.mem_applyFactSet]
       exists f; constructor; rw [List.mem_toSet]; exact f_mem; exact e_eq
-  . simp only [backtracking, backtrackFacts]
+  . simp only [backtrackFacts]
     rw [fresh_constant_remapping_h.right.right]
     simp only [mapped_body_map_swap, forbidden_constants_map_g_eq]
 
