ExistentialRules/ChaseSequence/Termination/RenameConstantsApart/PreTrigger.lean
@@ -17,7 +17,7 @@ This pretty much happens in the obvious way and apart from being technical, this
 
 public section
 
-variable {sig : Signature} [DecidableEq sig.C] [DecidableEq sig.V]
+variable {sig : Signature} [DecidableEq sig.P] [DecidableEq sig.C] [DecidableEq sig.V]
 
 namespace GroundSubstitution
 
@@ -55,77 +55,9 @@ theorem rename_constants_apart_for_vars_constants_fresh
       apply ih
       simp [new_forbidden, contra]
 
-variable [DecidableEq sig.P]
-
-theorem rename_constants_apart_for_vars_preserves_ruleId_validity [GetFreshInhabitant sig.C]
-    (subs : GroundSubstitution sig) (forbidden_constants : List sig.C) (vars : List sig.V) :
-    ∀ rl, ∀ v ∈ vars, (subs v).skolem_ruleIds_valid rl -> (subs.rename_constants_apart_for_vars forbidden_constants vars v).skolem_ruleIds_valid rl := by
-  intro rl v
-  induction vars generalizing forbidden_constants with
-  | nil => intros; contradiction
-  | cons hd tl ih =>
-    intro v_mem
-    rw [List.mem_cons] at v_mem
-    cases Decidable.em (v = hd) with
-    | inl v_eq =>
-      simp only [rename_constants_apart_for_vars, v_eq, ↓reduceIte]
-      apply GroundTerm.rename_constants_apart_preserves_ruleId_validity
-    | inr v_neq =>
-      simp only [rename_constants_apart_for_vars, v_neq, ↓reduceIte]
-      apply ih
-      cases v_mem with
-      | inl v_mem => contradiction
-      | inr v_mem => exact v_mem
-
-theorem rename_constants_apart_for_vars_preserves_disjIdx_validity [GetFreshInhabitant sig.C]
-    (subs : GroundSubstitution sig) (forbidden_constants : List sig.C) (vars : List sig.V) :
-    ∀ rl, ∀ v, (v_mem : v ∈ vars) -> (h : (subs v).skolem_ruleIds_valid rl) -> (subs v).skolem_disjIdx_valid rl h ->
-    (subs.rename_constants_apart_for_vars forbidden_constants vars v).skolem_disjIdx_valid rl
-      (subs.rename_constants_apart_for_vars_preserves_ruleId_validity forbidden_constants vars rl v v_mem h) := by
-  intro rl v
-  induction vars generalizing forbidden_constants with
-  | nil => intros; contradiction
-  | cons hd tl ih =>
-    intro v_mem
-    rw [List.mem_cons] at v_mem
-    cases Decidable.em (v = hd) with
-    | inl v_eq =>
-      simp only [rename_constants_apart_for_vars, v_eq, ↓reduceIte]
-      apply GroundTerm.rename_constants_apart_preserves_disjIdx_validity
-    | inr v_neq =>
-      simp only [rename_constants_apart_for_vars, v_neq, ↓reduceIte]
-      apply ih
-      cases v_mem with
-      | inl v_mem => contradiction
-      | inr v_mem => exact v_mem
-
-theorem rename_constants_apart_for_vars_preserves_rule_arity_validity [GetFreshInhabitant sig.C]
-    (subs : GroundSubstitution sig) (forbidden_constants : List sig.C) (vars : List sig.V) :
-    ∀ rl, ∀ v, (v_mem : v ∈ vars) -> (h : (subs v).skolem_ruleIds_valid rl) -> (subs v).skolem_rule_arity_valid rl h ->
-    (subs.rename_constants_apart_for_vars forbidden_constants vars v).skolem_rule_arity_valid rl
-      (subs.rename_constants_apart_for_vars_preserves_ruleId_validity forbidden_constants vars rl v v_mem h) := by
-  intro rl v
-  induction vars generalizing forbidden_constants with
-  | nil => intros; contradiction
-  | cons hd tl ih =>
-    intro v_mem
-    rw [List.mem_cons] at v_mem
-    cases Decidable.em (v = hd) with
-    | inl v_eq =>
-      simp only [rename_constants_apart_for_vars, v_eq, ↓reduceIte]
-      apply GroundTerm.rename_constants_apart_preserves_rule_arity_validity
-    | inr v_neq =>
-      simp only [rename_constants_apart_for_vars, v_neq, ↓reduceIte]
-      apply ih
-      cases v_mem with
-      | inl v_mem => contradiction
-      | inr v_mem => exact v_mem
-
 end GroundSubstitution
 
 namespace PreTrigger
-
-variable [DecidableEq sig.P]
 
 @[expose]
 def rename_constants_apart [GetFreshInhabitant sig.C] (trg : PreTrigger sig) (forbidden_constants : List sig.C) : PreTrigger sig :=
@@ -145,74 +77,6 @@ theorem rename_constants_apart_constants_fresh
   apply trg.subs.rename_constants_apart_for_vars_constants_fresh forbidden_constants trg.rule.body.vars.eraseDupsKeepRight v v_mem
   rw [← t_eq] at c_mem
   exact c_mem
-
-theorem rename_constants_apart_preserves_ruleId_validity [GetFreshInhabitant sig.C] (trg : PreTrigger sig) (forbidden_constants : List sig.C) :
-    ∀ rl, PreTrigger.skolem_ruleIds_valid rl trg ->
-    PreTrigger.skolem_ruleIds_valid rl (PreTrigger.rename_constants_apart trg forbidden_constants) := by
-  intro rl valid
-  unfold skolem_ruleIds_valid at *
-  intro t t_mem
-  rw [mem_terms_mapped_body_iff] at t_mem
-  cases t_mem with
-  | inl t_mem =>
-    rcases t_mem with ⟨c, c_mem, t_eq⟩
-    rw [← t_eq]
-    apply GroundTerm.skolem_ruleIds_valid_const
-  | inr t_mem =>
-    rcases t_mem with ⟨v, v_mem, t_eq⟩
-    rw [← t_eq]
-    apply trg.subs.rename_constants_apart_for_vars_preserves_ruleId_validity forbidden_constants trg.rule.body.vars.eraseDupsKeepRight rl v
-    . rw [List.mem_eraseDupsKeepRight]; exact v_mem
-    . apply valid
-      rw [mem_terms_mapped_body_iff]
-      apply Or.inr
-      exists v
-
-theorem rename_constants_apart_preserves_disjIdx_validity [GetFreshInhabitant sig.C] (trg : PreTrigger sig) (forbidden_constants : List sig.C) :
-    ∀ rl, (h : PreTrigger.skolem_ruleIds_valid rl trg) -> PreTrigger.skolem_disjIdx_valid rl trg h ->
-    PreTrigger.skolem_disjIdx_valid rl (PreTrigger.rename_constants_apart trg forbidden_constants)
-      (PreTrigger.rename_constants_apart_preserves_ruleId_validity trg forbidden_constants rl h) := by
-  intro rl h valid
-  unfold skolem_disjIdx_valid at *
-  intro t t_mem
-  rw [mem_terms_mapped_body_iff] at t_mem
-  cases t_mem with
-  | inl t_mem =>
-    rcases t_mem with ⟨c, c_mem, t_eq⟩
-    simp only [← t_eq]
-    apply GroundTerm.skolem_disjIdx_valid_const
-  | inr t_mem =>
-    rcases t_mem with ⟨v, v_mem, t_eq⟩
-    simp only [← t_eq]
-    apply trg.subs.rename_constants_apart_for_vars_preserves_disjIdx_validity forbidden_constants trg.rule.body.vars.eraseDupsKeepRight rl v
-    . rw [List.mem_eraseDupsKeepRight]; exact v_mem
-    . apply valid
-      rw [mem_terms_mapped_body_iff]
-      apply Or.inr
-      exists v
-
-theorem rename_constants_apart_preserves_rule_arity_validity [GetFreshInhabitant sig.C] (trg : PreTrigger sig) (forbidden_constants : List sig.C) :
-    ∀ rl, (h : PreTrigger.skolem_ruleIds_valid rl trg) -> PreTrigger.skolem_rule_arity_valid rl trg h ->
-    PreTrigger.skolem_rule_arity_valid rl (PreTrigger.rename_constants_apart trg forbidden_constants)
-      (PreTrigger.rename_constants_apart_preserves_ruleId_validity trg forbidden_constants rl h) := by
-  intro rl h valid
-  unfold skolem_rule_arity_valid at *
-  intro t t_mem
-  rw [mem_terms_mapped_body_iff] at t_mem
-  cases t_mem with
-  | inl t_mem =>
-    rcases t_mem with ⟨c, c_mem, t_eq⟩
-    simp only [← t_eq]
-    apply GroundTerm.skolem_rule_arity_valid_const
-  | inr t_mem =>
-    rcases t_mem with ⟨v, v_mem, t_eq⟩
-    simp only [← t_eq]
-    apply trg.subs.rename_constants_apart_for_vars_preserves_rule_arity_validity forbidden_constants trg.rule.body.vars.eraseDupsKeepRight rl v
-    . rw [List.mem_eraseDupsKeepRight]; exact v_mem
-    . apply valid
-      rw [mem_terms_mapped_body_iff]
-      apply Or.inr
-      exists v
 
 end PreTrigger
 
